Loom/Triple/SpecLemmas.lean
@@ -185,11 +185,11 @@ namespace Std.Do'
 open Lean.Order
 
 universe u v
-variable {m : Type u → Type v} {l : Type u} {e : Type u}
+variable {m : Type u → Type v} {Pred : Type u} {EPred : Type u}
 
 /-! # `Monad` -/
 
-variable [Monad m] [AssertionLang l] [ExceptAssertionLang e] [WPMonad m l e]
+variable [Monad m] [Assertion Pred] [Assertion EPred] [WP m Pred EPred]
 
 theorem Spec.pure' (a : α) (h : pre ⊑ post a) :
     Triple pre (Pure.pure (f := m) a) post epost :=
@@ -214,7 +214,7 @@ theorem Spec.bind (x : m α) (f : α → m β) :
 theorem Spec.map' (f : α → β) (x : m α)
     (h : Triple pre x (fun a => post (f a)) epost) :
     Triple pre (f <$> x) post epost :=
-  Triple.iff.mpr (PartialOrder.rel_trans (Triple.iff.mp h) (WPMonad.wp_map f x post epost))
+  Triple.iff.mpr (PartialOrder.rel_trans (Triple.iff.mp h) (WP.wp_map f x post epost))
 
 @[lspec]
 theorem Spec.map (f : α → β) (x : m α) :
@@ -224,7 +224,7 @@ theorem Spec.map (f : α → β) (x : m α) :
 theorem Spec.seq' (x : m (α → β)) (y : m α)
     (h : Triple pre x (fun f => wp y (fun a => post (f a)) epost) epost) :
     Triple pre (x <*> y) post epost :=
-  Triple.iff.mpr (PartialOrder.rel_trans (Triple.iff.mp h) (WPMonad.wp_seq x y post epost))
+  Triple.iff.mpr (PartialOrder.rel_trans (Triple.iff.mp h) (WP.wp_seq x y post epost))
 
 @[lspec]
 theorem Spec.seq (x : m (α → β)) (y : m α) :
@@ -234,26 +234,24 @@ theorem Spec.seq (x : m (α → β)) (y : m α) :
 /-! # `MonadLift` -/
 
 @[lspec]
-theorem Spec.monadLift_StateT (x : m α) (post : α → σ → l) :
+theorem Spec.monadLift_StateT (x : m α) (post : α → σ → Pred) :
     Triple (fun s => wp x (fun a => post a s) epost) (MonadLift.monadLift x : StateT σ m α) post epost :=
   Triple.iff.mpr (WP.monadLift_StateT_wp x post)
 
 @[lspec]
-theorem Spec.monadLift_ReaderT (x : m α) (post : α → ρ → l) :
+theorem Spec.monadLift_ReaderT (x : m α) (post : α → ρ → Pred) :
     Triple (fun r => wp x (fun a => post a r) epost) (MonadLift.monadLift x : ReaderT ρ m α) post epost :=
   Triple.iff.mpr (by rw [WP.monadLift_ReaderT_wp]; rfl)
 
 @[lspec]
-theorem Spec.monadLift_ExceptT (x : m α) (post : α → l) (epost : EPost.cons (ε → l) e) :
+theorem Spec.monadLift_ExceptT (x : m α) (post : α → Pred) (epost : EPost.cons (ε → Pred) EPred) :
     Triple (wp x post epost.tail) (MonadLift.monadLift x : ExceptT ε m α) post epost :=
   Triple.iff.mpr (WP.monadLift_ExceptT_wp x post epost)
 
-/-
 @[lspec]
-theorem Spec.monadLift_OptionT (x : m α) (post : α → l) (epost : e × l) :
-    Triple (wp x post epost.1) (MonadLift.monadLift x : OptionT m α) post epost :=
-  Triple.iff.mpr (monadLift_OptionT_wp x)
--/
+theorem Spec.monadLift_OptionT (x : m α) (post : α → Pred) (epost : EPost.cons Pred EPred) :
+    Triple (wp x post epost.tail) (MonadLift.monadLift x : OptionT m α) post epost :=
+  Triple.iff.mpr (WP.monadLift_OptionT_wp x)
 
 /-! # `MonadFunctor` -/
 
@@ -261,33 +259,31 @@ attribute [refl] PartialOrder.rel_refl
 
 @[lspec]
 theorem Spec.monadMap_StateT
-    (f : ∀{β}, m β → m β) {α} (x : StateT σ m α) (post : α → σ → l) :
+    (f : ∀{β}, m β → m β) {α} (x : StateT σ m α) (post : α → σ → Pred) :
     Triple (fun s => wp (f (x.run s)) (fun (a, s') => post a s') epost)
       (MonadFunctor.monadMap (m := m) f x : StateT σ m α) post epost :=
   Triple.iff.mpr (by rw [WP.monadMap_StateT_wp]; rfl)
 
 @[lspec]
 theorem Spec.monadMap_ReaderT
-    (f : ∀{β}, m β → m β) {α} (x : ReaderT ρ m α) (post : α → ρ → l) :
+    (f : ∀{β}, m β → m β) {α} (x : ReaderT ρ m α) (post : α → ρ → Pred) :
     Triple (fun r => wp (f (x.run r)) (fun a => post a r) epost)
       (MonadFunctor.monadMap (m := m) f x : ReaderT ρ m α) post epost :=
   Triple.iff.mpr (by rw [WP.monadMap_ReaderT_wp]; rfl)
 
 @[lspec]
 theorem Spec.monadMap_ExceptT
-    (f : ∀{β}, m β → m β) {α} (x : ExceptT ε m α) (post : α → l) (epost : EPost.cons (ε → l) e) :
+    (f : ∀{β}, m β → m β) {α} (x : ExceptT ε m α) (post : α → Pred) (epost : EPost.cons (ε → Pred) EPred) :
     Triple (wp (f x.run) (epost.pushExcept post) epost.tail)
       (MonadFunctor.monadMap (m := m) f x : ExceptT ε m α) post epost :=
   Triple.iff.mpr (by rw [WP.monadMap_ExceptT_wp])
 
-/-
 @[lspec]
 theorem Spec.monadMap_OptionT
-    (f : ∀{β}, m β → m β) {α} (x : OptionT m α) (post : α → l) (epost : e × l) :
-    Triple (wp (f x.run) (fun o => match o with | some a => post a | none => epost.2) epost.1)
+    (f : ∀{β}, m β → m β) {α} (x : OptionT m α) (post : α → Pred) (epost : EPost.cons Pred EPred) :
+    Triple (wp (f x.run) (epost.pushOption post) epost.tail)
       (MonadFunctor.monadMap (m := m) f x : OptionT m α) post epost :=
-  Triple.iff.mpr (by rw [monadMap_OptionT_wp]; rfl)
--/
+  Triple.iff.mpr (by rw [WP.monadMap_OptionT_wp])
 
 
 @[lspec]
@@ -300,59 +296,55 @@ theorem Spec.monadMap_refl (x : m α) :
 
 @[lspec]
 theorem Spec.liftWith_StateT
-    (f : (∀{β}, StateT σ m β → m (β × σ)) → m α) (post : α → σ → l) :
+    (f : (∀{β}, StateT σ m β → m (β × σ)) → m α) (post : α → σ → Pred) :
     Triple (fun s => wp (f (fun x => x.run s)) (fun a => post a s) epost)
       (MonadControl.liftWith (m:=m) f : StateT σ m α) post epost :=
-  Triple.iff.mpr (by intro s; simp [WP.liftWith_StateT_wp f]; apply WPMonad.wp_map'; ext; rfl)
+  Triple.iff.mpr (by intro s; simp [WP.liftWith_StateT_wp f]; apply WP.wp_map'; ext; rfl)
 
 @[lspec]
 theorem Spec.liftWith_ReaderT
-    (f : (∀{β}, ReaderT ρ m β → m β) → m α) (post : α → ρ → l) :
+    (f : (∀{β}, ReaderT ρ m β → m β) → m α) (post : α → ρ → Pred) :
     Triple (fun r => wp (f (fun x => x.run r)) (fun a => post a r) epost)
       (MonadControl.liftWith (m:=m) f : ReaderT ρ m α) post epost :=
   Triple.iff.mpr (by intro r; simp [WP.liftWith_ReaderT_wp f]; rfl)
 
 @[lspec]
 theorem Spec.liftWith_ExceptT
-    (f : (∀{β}, ExceptT ε m β → m (Except ε β)) → m α) (post : α → l) (epost : EPost.cons (ε → l) e) :
+    (f : (∀{β}, ExceptT ε m β → m (Except ε β)) → m α) (post : α → Pred) (epost : EPost.cons (ε → Pred) EPred) :
     Triple (wp (f (fun x => x.run)) post epost.tail)
       (MonadControl.liftWith (m:=m) f : ExceptT ε m α) post epost :=
-  Triple.iff.mpr (by simp [WP.liftWith_ExceptT_wp f]; apply WPMonad.wp_map'; ext; rfl)
+  Triple.iff.mpr (by simp [WP.liftWith_ExceptT_wp f]; apply WP.wp_map'; ext; rfl)
 
-/-
 @[lspec]
 theorem Spec.liftWith_OptionT
-    (f : (∀{β}, OptionT m β → m (Option β)) → m α) (post : α → l) (epost : e × l) :
-    Triple (wp (f (fun x => x.run)) post epost.1)
+    (f : (∀{β}, OptionT m β → m (Option β)) → m α) (post : α → Pred) (epost : EPost.cons Pred EPred) :
+    Triple (wp (f (fun x => x.run)) post epost.tail)
       (MonadControl.liftWith (m:=m) f : OptionT m α) post epost :=
   Triple.iff.mpr (WP.liftWith_OptionT_wp f)
--/
 
 @[lspec]
-theorem Spec.restoreM_StateT (x : m (α × σ)) (post : α → σ → l) :
+theorem Spec.restoreM_StateT (x : m (α × σ)) (post : α → σ → Pred) :
     Triple (fun _ => wp x (fun (a, s) => post a s) epost)
       (MonadControl.restoreM (m:=m) x : StateT σ m α) post epost :=
   Triple.iff.mpr (WP.restoreM_StateT_wp x)
 
 @[lspec]
-theorem Spec.restoreM_ReaderT (x : m α) (post : α → ρ → l) :
+theorem Spec.restoreM_ReaderT (x : m α) (post : α → ρ → Pred) :
     Triple (fun r => wp x (fun a => post a r) epost)
       (MonadControl.restoreM (m:=m) x : ReaderT ρ m α) post epost :=
   Triple.iff.mpr (by rw [WP.restoreM_ReaderT_wp]; rfl)
 
 @[lspec]
-theorem Spec.restoreM_ExceptT (x : m (@Except.{u, u} ε α)) (post : α → l) (epost : EPost.cons (ε → l) e) :
+theorem Spec.restoreM_ExceptT (x : m (@Except.{u, u} ε α)) (post : α → Pred) (epost : EPost.cons (ε → Pred) EPred) :
     Triple (wp x (epost.pushExcept post) epost.tail)
       (MonadControl.restoreM (m:=m) x : ExceptT ε m α) post epost :=
   Triple.iff.mpr (by rw [WP.restoreM_ExceptT_wp])
 
-/-
 @[lspec]
-theorem Spec.restoreM_OptionT (x : m (Option α)) (post : α → l) (epost : e × l) :
-    Triple (wp x (fun (o : Option α) => match o with | some a => post a | none => epost.2) epost.1)
+theorem Spec.restoreM_OptionT (x : m (Option α)) (post : α → Pred) (epost : EPost.cons Pred EPred) :
+    Triple (wp x (epost.pushOption post) epost.tail)
       (MonadControl.restoreM (m:=m) x : OptionT m α) post epost :=
-  Triple.iff.mpr (by rw [WP.restoreM_OptionT_wp]; rfl)
--/
+  Triple.iff.mpr (by rw [WP.restoreM_OptionT_wp])
 
 /-! # `MonadControlT` -/
 
@@ -374,19 +366,19 @@ theorem Spec.restoreM_refl (x : stM m m α) :
 /-! # `ReaderT` -/
 
 @[lspec]
-theorem Spec.read_ReaderT (post : ρ → ρ → l) :
+theorem Spec.read_ReaderT (post : ρ → ρ → Pred) :
     Triple (fun r => post r r)
       (MonadReaderOf.read : ReaderT ρ m ρ) post epost :=
   Triple.iff.mpr (by intro r; simpa [MonadReaderOf.read] using
-    (WPMonad.wp_pure (m := m) (x := r) (post := fun a => post a r) (epost := epost)))
+    (WP.wp_pure (m := m) (x := r) (post := fun a => post a r) (epost := epost)))
 @[lspec]
-theorem Spec.withReader_ReaderT (f : ρ → ρ) (x : ReaderT ρ m α) (post : α → ρ → l) :
+theorem Spec.withReader_ReaderT (f : ρ → ρ) (x : ReaderT ρ m α) (post : α → ρ → Pred) :
     Triple (fun r => wp x (fun a _ => post a r) epost (f r))
       (MonadWithReaderOf.withReader f x : ReaderT ρ m α) post epost :=
   Triple.iff.mpr (by rw [WP.withReader_ReaderT_wp]; rfl)
 
 @[lspec]
-theorem Spec.adapt_ReaderT (f : ρ → ρ') (x : ReaderT ρ' m α) (post : α → ρ → l) :
+theorem Spec.adapt_ReaderT (f : ρ → ρ') (x : ReaderT ρ' m α) (post : α → ρ → Pred) :
     Triple (fun r => wp x (fun a _ => post a r) epost (f r))
       (ReaderT.adapt f x : ReaderT ρ m α) post epost :=
   Triple.iff.mpr (by rw [WP.adapt_ReaderT_wp]; rfl)
@@ -394,33 +386,33 @@ theorem Spec.adapt_ReaderT (f : ρ → ρ') (x : ReaderT ρ' m α) (post : α �
 /-! # `StateT` -/
 
 @[lspec]
-theorem Spec.get_StateT (post : σ → σ → l) :
+theorem Spec.get_StateT (post : σ → σ → Pred) :
     Triple (fun s => post s s)
       (MonadStateOf.get : StateT σ m σ) post epost :=
   Triple.iff.mpr (by intro s; simpa [get_StateT] using
-    (WPMonad.wp_pure (m := m) (x := (s, s))
+    (WP.wp_pure (m := m) (x := (s, s))
       (post := fun x => post x.fst x.snd) (epost := epost)))
 
 @[lspec]
-theorem Spec.set_StateT (s : σ) (post : PUnit → σ → l) :
+theorem Spec.set_StateT (s : σ) (post : PUnit → σ → Pred) :
     Triple (fun _ => post ⟨⟩ s)
       (set s : StateT σ m PUnit) post epost :=
   Triple.iff.mpr (by intro _; simpa [MonadStateOf.set] using
-    (WPMonad.wp_pure (m := m) (x := (PUnit.unit, s))
+    (WP.wp_pure (m := m) (x := (PUnit.unit, s))
       (post := fun x => post x.fst x.snd) (epost := epost)))
 
 @[lspec]
-theorem Spec.modifyGet_StateT (f : σ → α × σ) (post : α → σ → l) :
+theorem Spec.modifyGet_StateT (f : σ → α × σ) (post : α → σ → Pred) :
     Triple (fun s => post (f s).1 (f s).2)
       (MonadStateOf.modifyGet f : StateT σ m α) post epost :=
   Triple.iff.mpr (by intro s; simpa [MonadStateOf.modifyGet] using
-    (WPMonad.wp_pure (m := m) (x := f s)
+    (WP.wp_pure (m := m) (x := f s)
       (post := fun x => post x.fst x.snd) (epost := epost)))
 
 /-! # `ExceptT` -/
 
 @[lspec]
-theorem Spec.run_ExceptT (x : ExceptT ε m α) (post : α → l) (epost : EPost.cons (ε → l) e) :
+theorem Spec.run_ExceptT (x : ExceptT ε m α) (post : α → Pred) (epost : EPost.cons (ε → Pred) EPred) :
     Triple (wp x post epost)
       (x.run : m (@Except.{u, u} ε α))
       (epost.pushExcept post)
@@ -428,27 +420,27 @@ theorem Spec.run_ExceptT (x : ExceptT ε m α) (post : α → l) (epost : EPost.
   Triple.iff.mpr (by simp [PartialOrder.rel_refl])
 
 @[lspec]
-theorem Spec.throw_ExceptT (err : ε) (post : α → l) (epost : EPost.cons (ε → l) e) :
+theorem Spec.throw_ExceptT (err : ε) (post : α → Pred) (epost : EPost.cons (ε → Pred) EPred) :
     Triple (epost.head err) (MonadExceptOf.throw err : ExceptT ε m α) post epost :=
   Triple.iff.mpr (by simpa [EPost.cons.pushExcept] using
-    (WPMonad.wp_pure (m := m) (x := Except.error err)
+    (WP.wp_pure (m := m) (x := Except.error err)
       (post := epost.pushExcept post)
       (epost := epost.tail)))
 
 @[lspec]
-theorem Spec.tryCatch_ExceptT (x : ExceptT ε m α) (h : ε → ExceptT ε m α) (post : α → l) (epost : EPost.cons (ε → l) e) :
+theorem Spec.tryCatch_ExceptT (x : ExceptT ε m α) (h : ε → ExceptT ε m α) (post : α → Pred) (epost : EPost.cons (ε → Pred) EPred) :
     Triple (wp x post ⟨fun e => wp (h e) post epost, epost.tail⟩)
       (MonadExceptOf.tryCatch x h : ExceptT ε m α) post epost :=
   Triple.iff.mpr (WP.tryCatch_ExceptT_wp x h)
 
 @[lspec]
-theorem Spec.orElse_ExceptT (x : ExceptT ε m α) (h : Unit → ExceptT ε m α) (post : α → l) (epost : EPost.cons (ε → l) e) :
+theorem Spec.orElse_ExceptT (x : ExceptT ε m α) (h : Unit → ExceptT ε m α) (post : α → Pred) (epost : EPost.cons (ε → Pred) EPred) :
     Triple (wp x post ⟨fun _ => wp (h ()) post epost, epost.tail⟩)
       (OrElse.orElse x h : ExceptT ε m α) post epost :=
   Triple.iff.mpr (WP.orElse_ExceptT_wp x h)
 
 @[lspec]
-theorem Spec.adapt_ExceptT (f : ε → ε') (x : ExceptT ε m α) (post : α → l) (epost : EPost.cons (ε' → l) e) :
+theorem Spec.adapt_ExceptT (f : ε → ε') (x : ExceptT ε m α) (post : α → Pred) (epost : EPost.cons (ε' → Pred) EPred) :
     Triple (wp x post ⟨fun e => epost.head (f e), epost.tail⟩)
       (ExceptT.adapt f x : ExceptT ε' m α) post epost :=
   Triple.iff.mpr (WP.adapt_ExceptT_wp f x)
@@ -470,55 +462,53 @@ theorem Spec.tryCatch_Except (x : Except ε α) (h : ε → Except ε α) :
 theorem Spec.orElse_Except (x : Except ε α) (h : Unit → Except ε α) :
     Triple (wp x post epost⟨fun (_ : ε) => wp (h ()) post epost⟩)
       (OrElse.orElse x h : Except ε α) post epost :=
-  Triple.iff.mpr (by simp only [wp, WPMonad.wpTrans, OrElse.orElse, MonadExcept.orElse]; cases x <;> rfl)
+  Triple.iff.mpr (by simp only [wp, WP.wpTrans, OrElse.orElse, MonadExcept.orElse]; cases x <;> rfl)
 
 /-! # `OptionT` -/
 
-/-
 @[lspec]
-theorem Spec.run_OptionT (x : OptionT m α) (post : α → l) (epost : e × l) :
+theorem Spec.run_OptionT (x : OptionT m α) (post : α → Pred) (epost : EPost.cons Pred EPred) :
     Triple (wp x post epost)
       (x.run : m (Option α))
-      (fun | some a => post a | none => epost.2)
-      epost.1 :=
-  Triple.iff.mpr (by rw [← OptionT_run_wp]; rfl)
+      (epost.pushOption post)
+      epost.tail :=
+  Triple.iff.mpr (by rw [← OptionT.apply_wp])
 
 @[lspec]
-theorem Spec.throw_OptionT (err : PUnit) (post : α → l) (epost : e × l) :
-    Triple epost.2 (MonadExceptOf.throw err : OptionT m α) post epost :=
-  Triple.iff.mpr (by rw [throw_OptionT_wp])
+theorem Spec.throw_OptionT (err : PUnit) (post : α → Pred) (epost : EPost.cons Pred EPred) :
+    Triple epost.head (MonadExceptOf.throw err : OptionT m α) post epost :=
+  Triple.iff.mpr (WP.throw_OptionT_wp err)
 
 @[lspec]
-theorem Spec.tryCatch_OptionT (x : OptionT m α) (h : PUnit → OptionT m α) (post : α → l) (epost : e × l) :
-    Triple (wp x post (epost.1, wp (h ⟨⟩) post epost))
+theorem Spec.tryCatch_OptionT (x : OptionT m α) (h : PUnit → OptionT m α) (post : α → Pred) (epost : EPost.cons Pred EPred) :
+    Triple (wp x post ⟨wp (h ⟨⟩) post epost, epost.tail⟩)
       (MonadExceptOf.tryCatch x h : OptionT m α) post epost :=
-  Triple.iff.mpr (tryCatch_OptionT_wp x h)
+  Triple.iff.mpr (WP.tryCatch_OptionT_wp x h)
 
 @[lspec]
-theorem Spec.orElse_OptionT (x : OptionT m α) (h : Unit → OptionT m α) (post : α → l) (epost : e × l) :
-    Triple (wp x post (epost.1, wp (h ()) post epost))
+theorem Spec.orElse_OptionT (x : OptionT m α) (h : Unit → OptionT m α) (post : α → Pred) (epost : EPost.cons Pred EPred) :
+    Triple (wp x post ⟨wp (h ()) post epost, epost.tail⟩)
       (OrElse.orElse x h : OptionT m α) post epost :=
-  Triple.iff.mpr (orElse_OptionT_wp x h)
+  Triple.iff.mpr (WP.orElse_OptionT_wp x h)
 
 /-! # `Option` -/
 
 @[lspec]
 theorem Spec.throw_Option (err : PUnit) :
     Triple epost (MonadExceptOf.throw err : Option α) post epost :=
-  Triple.iff.mpr (by rw [throw_Option_wp]; rfl)
+  Triple.iff.mpr (by rw [WP.throw_Option_wp]; rfl)
 
 @[lspec]
 theorem Spec.tryCatch_Option (x : Option α) (h : PUnit → Option α) :
     Triple (wp x post (wp (h ⟨⟩) post epost))
       (MonadExceptOf.tryCatch x h : Option α) post epost :=
-  Triple.iff.mpr (by rw [tryCatch_Option_wp]; rfl)
+  Triple.iff.mpr (by rw [WP.tryCatch_Option_wp]; rfl)
 
 @[lspec]
 theorem Spec.orElse_Option (x : Option α) (h : Unit → Option α) (post : α → Prop) (epost : Prop) :
     Triple (wp x post (wp (h ()) post epost))
       (OrElse.orElse x h : Option α) post epost :=
-  Triple.iff.mpr (by rw [orElse_Option_wp]; rfl)
--/
+  Triple.iff.mpr (by rw [WP.orElse_Option_wp]; rfl)
 
 /-! # `EStateM` -/
 
@@ -583,36 +573,34 @@ theorem Spec.tryCatch_MonadExcept [MonadExceptOf ε m] (x : m α) (h : ε → m 
   Triple.iff.mpr (by rw [WP.tryCatch_MonadExcept_wp])
 
 @[lspec]
-theorem Spec.throw_ReaderT [MonadExceptOf ε m] (err : ε) (post : α → ρ → l) :
+theorem Spec.throw_ReaderT [MonadExceptOf ε m] (err : ε) (post : α → ρ → Pred) :
     Triple (wp (MonadLift.monadLift (MonadExceptOf.throw (ε:=ε) err : m α) : ReaderT ρ m α) post epost)
       (MonadExceptOf.throw (ε:=ε) err : ReaderT ρ m α) post epost :=
   Triple.iff.mpr (by rw [WP.throw_ReaderT_lift_wp]; rfl)
 
 @[lspec]
-theorem Spec.throw_StateT [MonadExceptOf ε m] (err : ε) (post : α → σ → l) :
+theorem Spec.throw_StateT [MonadExceptOf ε m] (err : ε) (post : α → σ → Pred) :
     Triple (wp (MonadLift.monadLift (MonadExceptOf.throw (ε:=ε) err : m α) : StateT σ m α) post epost)
       (MonadExceptOf.throw (ε:=ε) err : StateT σ m α) post epost :=
   Triple.iff.mpr (by rw [WP.throw_StateT_lift_wp]; rfl)
 
 @[lspec]
-theorem Spec.throw_ExceptT_lift [MonadExceptOf ε m] (err : ε) (post : α → l) (epost : EPost.cons (ε' → l) e) :
+theorem Spec.throw_ExceptT_lift [MonadExceptOf ε m] (err : ε) (post : α → Pred) (epost : EPost.cons (ε' → Pred) EPred) :
     Triple (wp (MonadExceptOf.throw (ε:=ε) err : m (@Except.{u, u} ε' α))
         (fun r => match r with | .ok a => post a | .error e => epost.head e) epost.tail)
       (MonadExceptOf.throw (ε:=ε) err : ExceptT ε' m α) post epost :=
-  Triple.iff.mpr (by rw [WP.throw_lift_ExceptT_wp]; apply WPMonad.wp_cons; intro r; cases r <;> rfl)
+  Triple.iff.mpr (by rw [WP.throw_lift_ExceptT_wp]; apply WP.wp_consequence; intro r; cases r <;> rfl)
 
-/-
 @[lspec]
-theorem Spec.throw_Option_lift [MonadExceptOf ε m] (err : ε) (post : α → l) (epost : l × e) :
+theorem Spec.throw_Option_lift [MonadExceptOf ε m] (err : ε) (post : α → Pred) (epost : EPost.cons Pred EPred) :
     Triple (wp (MonadExceptOf.throw (ε:=ε) err : m (Option α))
-        (fun | some a => post a | none => epost.2) epost.1)
+        (epost.pushOption post) epost.tail)
       (MonadExceptOf.throw (ε:=ε) err : OptionT m α) post epost :=
-  Triple.iff.mpr (by rw [throw_lift_OptionT_wp]; apply WPMonad.wp_cons; intro r; cases r <;> rfl)
--/
+  Triple.iff.mpr (by rw [WP.throw_lift_OptionT_wp])
 
 @[lspec]
 theorem Spec.tryCatch_ReaderT [MonadExceptOf ε m] (x : ReaderT ρ m α) (h : ε → ReaderT ρ m α)
-    (post : α → ρ → l) :
+    (post : α → ρ → Pred) :
     Triple (fun r => wp (MonadExceptOf.tryCatch (ε:=ε) (x.run r) (fun e => (h e).run r) : m α)
         (fun a => post a r) epost)
       (MonadExceptOf.tryCatch (ε:=ε) x h : ReaderT ρ m α) post epost :=
@@ -620,7 +608,7 @@ theorem Spec.tryCatch_ReaderT [MonadExceptOf ε m] (x : ReaderT ρ m α) (h : ε
 
 @[lspec]
 theorem Spec.tryCatch_StateT [MonadExceptOf ε m] (x : StateT σ m α) (h : ε → StateT σ m α)
-    (post : α → σ → l) :
+    (post : α → σ → Pred) :
     Triple (fun s => wp (MonadExceptOf.tryCatch (ε:=ε) (x.run s) (fun e => (h e).run s) : m (α × σ))
         (fun (a, s') => post a s') epost)
       (MonadExceptOf.tryCatch (ε:=ε) x h : StateT σ m α) post epost :=
@@ -628,21 +616,19 @@ theorem Spec.tryCatch_StateT [MonadExceptOf ε m] (x : StateT σ m α) (h : ε �
 
 @[lspec]
 theorem Spec.tryCatch_ExceptT_lift [MonadExceptOf ε m] (x : ExceptT ε' m α) (h : ε → ExceptT ε' m α)
-    (post : α → l) (epost : EPost.cons (ε' → l) e) :
+    (post : α → Pred) (epost : EPost.cons (ε' → Pred) EPred) :
     Triple (wp (MonadExceptOf.tryCatch (ε:=ε) x h : m (@Except.{u, u} ε' α))
         (fun | .ok a => post a | .error e => epost.head e) epost.tail)
       (MonadExceptOf.tryCatch (ε:=ε) x h : ExceptT ε' m α) post epost :=
-  Triple.iff.mpr (by rw [WP.tryCatch_lift_ExceptT_wp]; apply WPMonad.wp_cons; intro r; cases r <;> rfl)
+  Triple.iff.mpr (by rw [WP.tryCatch_lift_ExceptT_wp]; apply WP.wp_consequence; intro r; cases r <;> rfl)
 
--- /-
--- @[lspec]
--- theorem Spec.tryCatch_OptionT_lift [MonadExceptOf ε m] (x : OptionT m α) (h : ε → OptionT m α)
---     (post : α → l) (epost : e × l) :
---     Triple (wp (MonadExceptOf.tryCatch (ε:=ε) x h : m (Option α))
---         (fun | some a => post a | none => epost.2) epost.1)
---       (MonadExceptOf.tryCatch (ε:=ε) x h : OptionT m α) post epost :=
---   Triple.iff.mpr (by rw [tryCatch_lift_OptionT_wp]; apply WPMonad.wp_cons; intro r; cases r <;> rfl)
--- -/
+@[lspec]
+theorem Spec.tryCatch_OptionT_lift [MonadExceptOf ε m] (x : OptionT m α) (h : ε → OptionT m α)
+    (post : α → Pred) (epost : EPost.cons Pred EPred) :
+    Triple (wp (MonadExceptOf.tryCatch (ε:=ε) x h : m (Option α))
+        (epost.pushOption post) epost.tail)
+      (MonadExceptOf.tryCatch (ε:=ε) x h : OptionT m α) post epost :=
+  Triple.iff.mpr (by rw [WP.tryCatch_lift_OptionT_wp])
 
 -- /-! # `MonadFunctorT` / `MonadControlT` transitivity -/
 
@@ -668,15 +654,6 @@ theorem Spec.liftWith_trans
   Triple.iff.mpr (by rw [WP.liftWith_trans_wp])
 
 
-@[lspec]
-theorem Spec.restoreM_trans
-    {n₁ : Type u → Type v} {n₂ : Type u → Type v}
-    [MonadControl n₁ m] [MonadControlT n₂ n₁]
-    (x : stM n₂ m α) :
-    Triple (wp (MonadControl.restoreM (m:=n₁) (MonadControlT.restoreM (m:=n₂) x) : m α) post epost)
-      (MonadControlT.restoreM (m:=n₂) x : m α) post epost :=
-  Triple.iff.mpr (by rw [WP.restoreM_trans_wp])
-
 end Std.Do'
 
 -- /-! # `ForIn` -/
@@ -685,8 +662,8 @@ namespace Std.Do'
 
 universe u₁ u₂ v
 
-variable {α : Type u₁} {β : Type (max u₁ u₂)} {m : Type (max u₁ u₂) → Type v} {l : Type (max u₁ u₂)} {e : Type (max u₁ u₂)}
-variable [Monad m] [AssertionLang l] [ExceptAssertionLang e] [WPMonad m l e]
+variable {α : Type u₁} {β : Type (max u₁ u₂)} {m : Type (max u₁ u₂) → Type v} {Pred : Type (max u₁ u₂)} {EPred : Type (max u₁ u₂)}
+variable [Monad m] [Assertion Pred] [Assertion EPred] [WP m Pred EPred]
 
 /--
 The type of loop invariants used by the specifications of `for ... in ...` loops.
@@ -695,17 +672,17 @@ A loop invariant is a pair of:
 * An exception postcondition `e`.
 -/
 abbrev Invariant {α : Type u₁} (xs : List α) (β : Type u₂)
-    (l : Type (max u₁ u₂)) :=
-  (List.Cursor xs × β → l)
+    (Pred : Type (max u₁ u₂)) :=
+  (List.Cursor xs × β → Pred)
 
 set_option linter.missingDocs false in
-abbrev eInvariant (e : Type u) := e
+abbrev eInvariant (EPred : Type u) := EPred
 
 @[lspec]
 theorem Spec.forIn'_list
     {xs : List α} {init : β} {f : (a : α) → a ∈ xs → β → m (ForInStep β)}
-    (inv : Invariant xs β l)
-    (eInv : e)
+    (inv : Invariant xs β Pred)
+    (eInv : EPred)
     (step : ∀ pref cur suff (h : xs = pref ++ cur :: suff) b,
       Triple
         (inv (⟨pref, cur::suff, h.symm⟩, b))
@@ -747,8 +724,8 @@ theorem Spec.forIn'_list
 @[lspec]
 theorem Spec.forIn'_list_const_inv
     {xs : List α} {init : β} {f : (a : α) → a ∈ xs → β → m (ForInStep β)}
-    {inv : (β → l)}
-    {eInv : e}
+    {inv : (β → Pred)}
+    {eInv : EPred}
     (step : ∀ x (hx : x ∈ xs) b,
       Triple
         (inv b)
@@ -763,8 +740,8 @@ theorem Spec.forIn'_list_const_inv
 @[lspec]
 theorem Spec.forIn_list
     {xs : List α} {init : β} {f : α → β → m (ForInStep β)}
-    (inv : Invariant xs β l)
-    (eInv : e)
+    (inv : Invariant xs β Pred)
+    (eInv : EPred)
     (step : ∀ pref cur suff (h : xs = pref ++ cur :: suff) b,
       Triple
         (inv (⟨pref, cur::suff, h.symm⟩, b))
@@ -785,8 +762,8 @@ theorem Spec.forIn_list
 @[lspec]
 theorem Spec.forIn_list_const_inv
     {xs : List α} {init : β} {f : α → β → m (ForInStep β)}
-    {inv : (β → l)}
-    {eInv : e}
+    {inv : (β → Pred)}
+    {eInv : EPred}
     (step : ∀ hd b,
       Triple
         (inv b)
@@ -799,8 +776,8 @@ theorem Spec.forIn_list_const_inv
 @[lspec]
 theorem Spec.foldlM_list [LawfulMonad m]
     {xs : List α} {init : β} {f : β → α → m β}
-    (inv : Invariant xs β l)
-    (eInv : e)
+    (inv : Invariant xs β Pred)
+    (eInv : EPred)
     (step : ∀ pref cur suff (h : xs = pref ++ cur :: suff) b,
       Triple
         (inv (⟨pref, cur::suff, h.symm⟩, b))
@@ -823,8 +800,8 @@ theorem Spec.foldlM_list [LawfulMonad m]
 @[lspec]
 theorem Spec.foldlM_list_const_inv [LawfulMonad m]
     {xs : List α} {init : β} {f : β → α → m β}
-    {inv : (β → l)}
-    {eInv : e}
+    {inv : (β → Pred)}
+    {eInv : EPred}
     (step : ∀ hd b,
       Triple
         (inv b)
@@ -835,11 +812,11 @@ theorem Spec.foldlM_list_const_inv [LawfulMonad m]
     Spec.foldlM_list (fun p => inv p.2) eInv (fun _p c _s _h b => step c b)
 
 @[lspec]
-theorem Spec.forIn'_range {β : Type u} {m : Type u → Type v} {l : Type u} {e : Type u}
-    [Monad m] [AssertionLang l] [ExceptAssertionLang e] [WPMonad m l e]
+theorem Spec.forIn'_range {β : Type u} {m : Type u → Type v} {Pred : Type u} {EPred : Type u}
+    [Monad m] [Assertion Pred] [Assertion EPred] [WP m Pred EPred]
     {xs : Std.Legacy.Range} {init : β} {f : (a : Nat) → a ∈ xs → β → m (ForInStep β)}
-    (inv : Invariant xs.toList β l)
-    (eInv : e)
+    (inv : Invariant xs.toList β Pred)
+    (eInv : EPred)
     (step : ∀ pref cur suff (h : xs.toList = pref ++ cur :: suff) b,
       Triple
         (inv (⟨pref, cur::suff, h.symm⟩, b))
@@ -857,11 +834,11 @@ theorem Spec.forIn'_range {β : Type u} {m : Type u → Type v} {l : Type u} {e 
   exact Spec.forIn'_list inv eInv (fun c hcur b => step c hcur b)
 
 @[lspec]
-theorem Spec.forIn_range {β : Type u} {m : Type u → Type v} {l : Type u} {e : Type u}
-    [Monad m] [AssertionLang l] [ExceptAssertionLang e] [WPMonad m l e]
+theorem Spec.forIn_range {β : Type u} {m : Type u → Type v} {Pred : Type u} {EPred : Type u}
+    [Monad m] [Assertion Pred] [Assertion EPred] [WP m Pred EPred]
     {xs : Std.Legacy.Range} {init : β} {f : Nat → β → m (ForInStep β)}
-    (inv : Invariant xs.toList β l)
-    (eInv : e)
+    (inv : Invariant xs.toList β Pred)
+    (eInv : EPred)
     (step : ∀ pref cur suff (h : xs.toList = pref ++ cur :: suff) b,
       Triple
         (inv (⟨pref, cur::suff, h.symm⟩, b))
@@ -880,13 +857,13 @@ theorem Spec.forIn_range {β : Type u} {m : Type u → Type v} {l : Type u} {e :
 
 open Std Std.PRange in
 @[lspec]
-theorem Spec.forIn'_rcc {α β : Type u} {m : Type u → Type v} {l : Type u} {e : Type u}
-    [Monad m] [AssertionLang l] [ExceptAssertionLang e] [WPMonad m l e] [LawfulMonad m]
+theorem Spec.forIn'_rcc {α β : Type u} {m : Type u → Type v} {Pred : Type u} {EPred : Type u}
+    [Monad m] [Assertion Pred] [Assertion EPred] [WP m Pred EPred] [LawfulMonad m]
     [LE α] [DecidableLE α] [UpwardEnumerable α] [Rxc.IsAlwaysFinite α]
     [LawfulUpwardEnumerable α] [LawfulUpwardEnumerableLE α]
     {xs : Rcc α} {init : β} {f : (a : α) → a ∈ xs → β → m (ForInStep β)}
-    (inv : Invariant xs.toList β l)
-    (eInv : e)
+    (inv : Invariant xs.toList β Pred)
+    (eInv : EPred)
     (step : ∀ pref cur suff (h : xs.toList = pref ++ cur :: suff) b,
       Triple
         (inv (⟨pref, cur::suff, h.symm⟩, b))
@@ -905,13 +882,13 @@ theorem Spec.forIn'_rcc {α β : Type u} {m : Type u → Type v} {l : Type u} {e
 
 open Std Std.PRange in
 @[lspec]
-theorem Spec.forIn_rcc {α β : Type u} {m : Type u → Type v} {l : Type u} {e : Type u}
-    [Monad m] [AssertionLang l] [ExceptAssertionLang e] [WPMonad m l e] [LawfulMonad m]
+theorem Spec.forIn_rcc {α β : Type u} {m : Type u → Type v} {Pred : Type u} {EPred : Type u}
+    [Monad m] [Assertion Pred] [Assertion EPred] [WP m Pred EPred] [LawfulMonad m]
     [LE α] [DecidableLE α] [UpwardEnumerable α] [Rxc.IsAlwaysFinite α]
     [LawfulUpwardEnumerable α] [LawfulUpwardEnumerableLE α]
     {xs : Rcc α} {init : β} {f : α → β → m (ForInStep β)}
-    (inv : Invariant xs.toList β l)
-    (eInv : e)
+    (inv : Invariant xs.toList β Pred)
+    (eInv : EPred)
     (step : ∀ pref cur suff (h : xs.toList = pref ++ cur :: suff) b,
       Triple
         (inv (⟨pref, cur::suff, h.symm⟩, b))
@@ -930,13 +907,13 @@ theorem Spec.forIn_rcc {α β : Type u} {m : Type u → Type v} {l : Type u} {e 
 
 open Std Std.PRange in
 @[lspec]
-theorem Spec.forIn'_rco {α β : Type u} {m : Type u → Type v} {l : Type u} {e : Type u}
-    [Monad m] [AssertionLang l] [ExceptAssertionLang e] [WPMonad m l e] [LawfulMonad m]
+theorem Spec.forIn'_rco {α β : Type u} {m : Type u → Type v} {Pred : Type u} {EPred : Type u}
+    [Monad m] [Assertion Pred] [Assertion EPred] [WP m Pred EPred] [LawfulMonad m]
     [LE α] [LT α] [DecidableLT α] [UpwardEnumerable α] [Rxo.IsAlwaysFinite α]
     [LawfulUpwardEnumerable α] [LawfulUpwardEnumerableLE α] [LawfulUpwardEnumerableLT α]
     {xs : Rco α} {init : β} {f : (a : α) → a ∈ xs → β → m (ForInStep β)}
-    (inv : Invariant xs.toList β l)
-    (eInv : e)
+    (inv : Invariant xs.toList β Pred)
+    (eInv : EPred)
     (step : ∀ pref cur suff (h : xs.toList = pref ++ cur :: suff) b,
       Triple
         (inv (⟨pref, cur::suff, h.symm⟩, b))
@@ -955,13 +932,13 @@ theorem Spec.forIn'_rco {α β : Type u} {m : Type u → Type v} {l : Type u} {e
 
 open Std Std.PRange in
 @[lspec]
-theorem Spec.forIn_rco {α β : Type u} {m : Type u → Type v} {l : Type u} {e : Type u}
-    [Monad m] [AssertionLang l] [ExceptAssertionLang e] [WPMonad m l e] [LawfulMonad m]
+theorem Spec.forIn_rco {α β : Type u} {m : Type u → Type v} {Pred : Type u} {EPred : Type u}
+    [Monad m] [Assertion Pred] [Assertion EPred] [WP m Pred EPred] [LawfulMonad m]
     [LE α] [LT α] [DecidableLT α] [UpwardEnumerable α] [Rxo.IsAlwaysFinite α]
     [LawfulUpwardEnumerable α] [LawfulUpwardEnumerableLE α] [LawfulUpwardEnumerableLT α]
     {xs : Rco α} {init : β} {f : α → β → m (ForInStep β)}
-    (inv : Invariant xs.toList β l)
-    (eInv : e)
+    (inv : Invariant xs.toList β Pred)
+    (eInv : EPred)
     (step : ∀ pref cur suff (h : xs.toList = pref ++ cur :: suff) b,
       Triple
         (inv (⟨pref, cur::suff, h.symm⟩, b))
@@ -980,13 +957,13 @@ theorem Spec.forIn_rco {α β : Type u} {m : Type u → Type v} {l : Type u} {e 
 
 open Std Std.PRange in
 @[lspec]
-theorem Spec.forIn'_rci {α β : Type u} {m : Type u → Type v} {l : Type u} {e : Type u}
-    [Monad m] [AssertionLang l] [ExceptAssertionLang e] [WPMonad m l e] [LawfulMonad m]
+theorem Spec.forIn'_rci {α β : Type u} {m : Type u → Type v} {Pred : Type u} {EPred : Type u}
+    [Monad m] [Assertion Pred] [Assertion EPred] [WP m Pred EPred] [LawfulMonad m]
     [LE α] [UpwardEnumerable α] [Rxi.IsAlwaysFinite α]
     [LawfulUpwardEnumerable α] [LawfulUpwardEnumerableLE α]
     {xs : Rci α} {init : β} {f : (a : α) → a ∈ xs → β → m (ForInStep β)}
-    (inv : Invariant xs.toList β l)
-    (eInv : e)
+    (inv : Invariant xs.toList β Pred)
+    (eInv : EPred)
     (step : ∀ pref cur suff (h : xs.toList = pref ++ cur :: suff) b,
       Triple
         (inv (⟨pref, cur::suff, h.symm⟩, b))
@@ -1005,13 +982,13 @@ theorem Spec.forIn'_rci {α β : Type u} {m : Type u → Type v} {l : Type u} {e
 
 open Std Std.PRange in
 @[lspec]
-theorem Spec.forIn_rci {α β : Type u} {m : Type u → Type v} {l : Type u} {e : Type u}
-    [Monad m] [AssertionLang l] [ExceptAssertionLang e] [WPMonad m l e] [LawfulMonad m]
+theorem Spec.forIn_rci {α β : Type u} {m : Type u → Type v} {Pred : Type u} {EPred : Type u}
+    [Monad m] [Assertion Pred] [Assertion EPred] [WP m Pred EPred] [LawfulMonad m]
     [LE α] [UpwardEnumerable α] [Rxi.IsAlwaysFinite α]
     [LawfulUpwardEnumerable α] [LawfulUpwardEnumerableLE α]
     {xs : Rci α} {init : β} {f : α → β → m (ForInStep β)}
-    (inv : Invariant xs.toList β l)
-    (eInv : e)
+    (inv : Invariant xs.toList β Pred)
+    (eInv : EPred)
     (step : ∀ pref cur suff (h : xs.toList = pref ++ cur :: suff) b,
       Triple
         (inv (⟨pref, cur::suff, h.symm⟩, b))
@@ -1030,13 +1007,13 @@ theorem Spec.forIn_rci {α β : Type u} {m : Type u → Type v} {l : Type u} {e 
 
 open Std Std.PRange in
 @[lspec]
-theorem Spec.forIn'_roc {α β : Type u} {m : Type u → Type v} {l : Type u} {e : Type u}
-    [Monad m] [AssertionLang l] [ExceptAssertionLang e] [WPMonad m l e] [LawfulMonad m]
+theorem Spec.forIn'_roc {α β : Type u} {m : Type u → Type v} {Pred : Type u} {EPred : Type u}
+    [Monad m] [Assertion Pred] [Assertion EPred] [WP m Pred EPred] [LawfulMonad m]
     [LE α] [DecidableLE α] [LT α] [UpwardEnumerable α] [Rxc.IsAlwaysFinite α]
     [LawfulUpwardEnumerable α] [LawfulUpwardEnumerableLE α] [LawfulUpwardEnumerableLT α]
     {xs : Roc α} {init : β} {f : (a : α) → a ∈ xs → β → m (ForInStep β)}
-    (inv : Invariant xs.toList β l)
-    (eInv : e)
+    (inv : Invariant xs.toList β Pred)
+    (eInv : EPred)
     (step : ∀ pref cur suff (h : xs.toList = pref ++ cur :: suff) b,
       Triple
         (inv (⟨pref, cur::suff, h.symm⟩, b))
@@ -1055,13 +1032,13 @@ theorem Spec.forIn'_roc {α β : Type u} {m : Type u → Type v} {l : Type u} {e
 
 open Std Std.PRange in
 @[lspec]
-theorem Spec.forIn_roc {α β : Type u} {m : Type u → Type v} {l : Type u} {e : Type u}
-    [Monad m] [AssertionLang l] [ExceptAssertionLang e] [WPMonad m l e] [LawfulMonad m]
+theorem Spec.forIn_roc {α β : Type u} {m : Type u → Type v} {Pred : Type u} {EPred : Type u}
+    [Monad m] [Assertion Pred] [Assertion EPred] [WP m Pred EPred] [LawfulMonad m]
     [LE α] [DecidableLE α] [LT α] [UpwardEnumerable α] [Rxc.IsAlwaysFinite α]
     [LawfulUpwardEnumerable α] [LawfulUpwardEnumerableLE α] [LawfulUpwardEnumerableLT α]
     {xs : Roc α} {init : β} {f : α → β → m (ForInStep β)}
-    (inv : Invariant xs.toList β l)
-    (eInv : e)
+    (inv : Invariant xs.toList β Pred)
+    (eInv : EPred)
     (step : ∀ pref cur suff (h : xs.toList = pref ++ cur :: suff) b,
       Triple
         (inv (⟨pref, cur::suff, h.symm⟩, b))
@@ -1080,13 +1057,13 @@ theorem Spec.forIn_roc {α β : Type u} {m : Type u → Type v} {l : Type u} {e 
 
 open Std Std.PRange in
 @[lspec]
-theorem Spec.forIn'_roo {α β : Type u} {m : Type u → Type v} {l : Type u} {e : Type u}
-    [Monad m] [AssertionLang l] [ExceptAssertionLang e] [WPMonad m l e] [LawfulMonad m]
+theorem Spec.forIn'_roo {α β : Type u} {m : Type u → Type v} {Pred : Type u} {EPred : Type u}
+    [Monad m] [Assertion Pred] [Assertion EPred] [WP m Pred EPred] [LawfulMonad m]
     [LT α] [DecidableLT α] [UpwardEnumerable α] [Rxo.IsAlwaysFinite α]
     [LawfulUpwardEnumerable α] [LawfulUpwardEnumerableLT α]
     {xs : Roo α} {init : β} {f : (a : α) → a ∈ xs → β → m (ForInStep β)}
-    (inv : Invariant xs.toList β l)
-    (eInv : e)
+    (inv : Invariant xs.toList β Pred)
+    (eInv : EPred)
     (step : ∀ pref cur suff (h : xs.toList = pref ++ cur :: suff) b,
       Triple
         (inv (⟨pref, cur::suff, h.symm⟩, b))
@@ -1105,13 +1082,13 @@ theorem Spec.forIn'_roo {α β : Type u} {m : Type u → Type v} {l : Type u} {e
 
 open Std Std.PRange in
 @[lspec]
-theorem Spec.forIn_roo {α β : Type u} {m : Type u → Type v} {l : Type u} {e : Type u}
-    [Monad m] [AssertionLang l] [ExceptAssertionLang e] [WPMonad m l e] [LawfulMonad m]
+theorem Spec.forIn_roo {α β : Type u} {m : Type u → Type v} {Pred : Type u} {EPred : Type u}
+    [Monad m] [Assertion Pred] [Assertion EPred] [WP m Pred EPred] [LawfulMonad m]
     [LT α] [DecidableLT α] [UpwardEnumerable α] [Rxo.IsAlwaysFinite α]
     [LawfulUpwardEnumerable α] [LawfulUpwardEnumerableLT α]
     {xs : Roo α} {init : β} {f : α → β → m (ForInStep β)}
-    (inv : Invariant xs.toList β l)
-    (eInv : e)
+    (inv : Invariant xs.toList β Pred)
+    (eInv : EPred)
     (step : ∀ pref cur suff (h : xs.toList = pref ++ cur :: suff) b,
       Triple
         (inv (⟨pref, cur::suff, h.symm⟩, b))
@@ -1130,13 +1107,13 @@ theorem Spec.forIn_roo {α β : Type u} {m : Type u → Type v} {l : Type u} {e 
 
 open Std Std.PRange in
 @[lspec]
-theorem Spec.forIn'_roi {α β : Type u} {m : Type u → Type v} {l : Type u} {e : Type u}
-    [Monad m] [AssertionLang l] [ExceptAssertionLang e] [WPMonad m l e] [LawfulMonad m]
+theorem Spec.forIn'_roi {α β : Type u} {m : Type u → Type v} {Pred : Type u} {EPred : Type u}
+    [Monad m] [Assertion Pred] [Assertion EPred] [WP m Pred EPred] [LawfulMonad m]
     [LT α] [DecidableLT α] [UpwardEnumerable α] [Rxi.IsAlwaysFinite α]
     [LawfulUpwardEnumerable α] [LawfulUpwardEnumerableLT α]
     {xs : Roi α} {init : β} {f : (a : α) → a ∈ xs → β → m (ForInStep β)}
-    (inv : Invariant xs.toList β l)
-    (eInv : e)
+    (inv : Invariant xs.toList β Pred)
+    (eInv : EPred)
     (step : ∀ pref cur suff (h : xs.toList = pref ++ cur :: suff) b,
       Triple
         (inv (⟨pref, cur::suff, h.symm⟩, b))
@@ -1155,13 +1132,13 @@ theorem Spec.forIn'_roi {α β : Type u} {m : Type u → Type v} {l : Type u} {e
 
 open Std Std.PRange in
 @[lspec]
-theorem Spec.forIn_roi {α β : Type u} {m : Type u → Type v} {l : Type u} {e : Type u}
-    [Monad m] [AssertionLang l] [ExceptAssertionLang e] [WPMonad m l e] [LawfulMonad m]
+theorem Spec.forIn_roi {α β : Type u} {m : Type u → Type v} {Pred : Type u} {EPred : Type u}
+    [Monad m] [Assertion Pred] [Assertion EPred] [WP m Pred EPred] [LawfulMonad m]
     [LT α] [DecidableLT α] [UpwardEnumerable α] [Rxi.IsAlwaysFinite α]
     [LawfulUpwardEnumerable α] [LawfulUpwardEnumerableLT α]
     {xs : Roi α} {init : β} {f : α → β → m (ForInStep β)}
-    (inv : Invariant xs.toList β l)
-    (eInv : e)
+    (inv : Invariant xs.toList β Pred)
+    (eInv : EPred)
     (step : ∀ pref cur suff (h : xs.toList = pref ++ cur :: suff) b,
       Triple
         (inv (⟨pref, cur::suff, h.symm⟩, b))
@@ -1180,13 +1157,13 @@ theorem Spec.forIn_roi {α β : Type u} {m : Type u → Type v} {l : Type u} {e 
 
 open Std Std.PRange in
 @[lspec]
-theorem Spec.forIn'_ric {α β : Type u} {m : Type u → Type v} {l : Type u} {e : Type u}
-    [Monad m] [AssertionLang l] [ExceptAssertionLang e] [WPMonad m l e] [LawfulMonad m]
+theorem Spec.forIn'_ric {α β : Type u} {m : Type u → Type v} {Pred : Type u} {EPred : Type u}
+    [Monad m] [Assertion Pred] [Assertion EPred] [WP m Pred EPred] [LawfulMonad m]
     [Least? α] [LE α] [DecidableLE α] [UpwardEnumerable α] [Rxc.IsAlwaysFinite α]
     [LawfulUpwardEnumerable α] [LawfulUpwardEnumerableLeast? α] [LawfulUpwardEnumerableLE α]
     {xs : Ric α} {init : β} {f : (a : α) → a ∈ xs → β → m (ForInStep β)}
-    (inv : Invariant xs.toList β l)
-    (eInv : e)
+    (inv : Invariant xs.toList β Pred)
+    (eInv : EPred)
     (step : ∀ pref cur suff (h : xs.toList = pref ++ cur :: suff) b,
       Triple
         (inv (⟨pref, cur::suff, h.symm⟩, b))
@@ -1205,13 +1182,13 @@ theorem Spec.forIn'_ric {α β : Type u} {m : Type u → Type v} {l : Type u} {e
 
 open Std Std.PRange in
 @[lspec]
-theorem Spec.forIn_ric {α β : Type u} {m : Type u → Type v} {l : Type u} {e : Type u}
-    [Monad m] [AssertionLang l] [ExceptAssertionLang e] [WPMonad m l e] [LawfulMonad m]
+theorem Spec.forIn_ric {α β : Type u} {m : Type u → Type v} {Pred : Type u} {EPred : Type u}
+    [Monad m] [Assertion Pred] [Assertion EPred] [WP m Pred EPred] [LawfulMonad m]
     [Least? α] [LE α] [DecidableLE α] [UpwardEnumerable α] [Rxc.IsAlwaysFinite α]
     [LawfulUpwardEnumerable α] [LawfulUpwardEnumerableLeast? α] [LawfulUpwardEnumerableLE α]
     {xs : Ric α} {init : β} {f : α → β → m (ForInStep β)}
-    (inv : Invariant xs.toList β l)
-    (eInv : e)
+    (inv : Invariant xs.toList β Pred)
+    (eInv : EPred)
     (step : ∀ pref cur suff (h : xs.toList = pref ++ cur :: suff) b,
       Triple
         (inv (⟨pref, cur::suff, h.symm⟩, b))
@@ -1230,13 +1207,13 @@ theorem Spec.forIn_ric {α β : Type u} {m : Type u → Type v} {l : Type u} {e 
 
 open Std Std.PRange in
 @[lspec]
-theorem Spec.forIn'_rio {α β : Type u} {m : Type u → Type v} {l : Type u} {e : Type u}
-    [Monad m] [AssertionLang l] [ExceptAssertionLang e] [WPMonad m l e] [LawfulMonad m]
+theorem Spec.forIn'_rio {α β : Type u} {m : Type u → Type v} {Pred : Type u} {EPred : Type u}
+    [Monad m] [Assertion Pred] [Assertion EPred] [WP m Pred EPred] [LawfulMonad m]
     [Least? α] [LT α] [DecidableLT α] [UpwardEnumerable α] [Rxo.IsAlwaysFinite α]
     [LawfulUpwardEnumerable α] [LawfulUpwardEnumerableLeast? α] [LawfulUpwardEnumerableLT α]
     {xs : Rio α} {init : β} {f : (a : α) → a ∈ xs → β → m (ForInStep β)}
-    (inv : Invariant xs.toList β l)
-    (eInv : e)
+    (inv : Invariant xs.toList β Pred)
+    (eInv : EPred)
     (step : ∀ pref cur suff (h : xs.toList = pref ++ cur :: suff) b,
       Triple
         (inv (⟨pref, cur::suff, h.symm⟩, b))
@@ -1255,13 +1232,13 @@ theorem Spec.forIn'_rio {α β : Type u} {m : Type u → Type v} {l : Type u} {e
 
 open Std Std.PRange in
 @[lspec]
-theorem Spec.forIn_rio {α β : Type u} {m : Type u → Type v} {l : Type u} {e : Type u}
-    [Monad m] [AssertionLang l] [ExceptAssertionLang e] [WPMonad m l e] [LawfulMonad m]
+theorem Spec.forIn_rio {α β : Type u} {m : Type u → Type v} {Pred : Type u} {EPred : Type u}
+    [Monad m] [Assertion Pred] [Assertion EPred] [WP m Pred EPred] [LawfulMonad m]
     [Least? α] [LT α] [DecidableLT α] [UpwardEnumerable α] [Rxo.IsAlwaysFinite α]
     [LawfulUpwardEnumerable α] [LawfulUpwardEnumerableLeast? α] [LawfulUpwardEnumerableLT α]
     {xs : Rio α} {init : β} {f : α → β → m (ForInStep β)}
-    (inv : Invariant xs.toList β l)
-    (eInv : e)
+    (inv : Invariant xs.toList β Pred)
+    (eInv : EPred)
     (step : ∀ pref cur suff (h : xs.toList = pref ++ cur :: suff) b,
       Triple
         (inv (⟨pref, cur::suff, h.symm⟩, b))
@@ -1280,13 +1257,13 @@ theorem Spec.forIn_rio {α β : Type u} {m : Type u → Type v} {l : Type u} {e 
 
 open Std Std.PRange in
 @[lspec]
-theorem Spec.forIn'_rii {α β : Type u} {m : Type u → Type v} {l : Type u} {e : Type u}
-    [Monad m] [AssertionLang l] [ExceptAssertionLang e] [WPMonad m l e] [LawfulMonad m]
+theorem Spec.forIn'_rii {α β : Type u} {m : Type u → Type v} {Pred : Type u} {EPred : Type u}
+    [Monad m] [Assertion Pred] [Assertion EPred] [WP m Pred EPred] [LawfulMonad m]
     [Least? α] [UpwardEnumerable α] [Rxi.IsAlwaysFinite α]
     [LawfulUpwardEnumerable α] [LawfulUpwardEnumerableLeast? α]
     {xs : Rii α} {init : β} {f : (a : α) → a ∈ xs → β → m (ForInStep β)}
-    (inv : Invariant xs.toList β l)
-    (eInv : e)
+    (inv : Invariant xs.toList β Pred)
+    (eInv : EPred)
     (step : ∀ pref cur suff (h : xs.toList = pref ++ cur :: suff) b,
       Triple
         (inv (⟨pref, cur::suff, h.symm⟩, b))
@@ -1305,13 +1282,13 @@ theorem Spec.forIn'_rii {α β : Type u} {m : Type u → Type v} {l : Type u} {e
 
 open Std Std.PRange in
 @[lspec]
-theorem Spec.forIn_rii {α β : Type u} {m : Type u → Type v} {l : Type u} {e : Type u}
-    [Monad m] [AssertionLang l] [ExceptAssertionLang e] [WPMonad m l e] [LawfulMonad m]
+theorem Spec.forIn_rii {α β : Type u} {m : Type u → Type v} {Pred : Type u} {EPred : Type u}
+    [Monad m] [Assertion Pred] [Assertion EPred] [WP m Pred EPred] [LawfulMonad m]
     [Least? α] [UpwardEnumerable α] [Rxi.IsAlwaysFinite α]
     [LawfulUpwardEnumerable α] [LawfulUpwardEnumerableLeast? α]
     {xs : Rii α} {init : β} {f : α → β → m (ForInStep β)}
-    (inv : Invariant xs.toList β l)
-    (eInv : e)
+    (inv : Invariant xs.toList β Pred)
+    (eInv : EPred)
     (step : ∀ pref cur suff (h : xs.toList = pref ++ cur :: suff) b,
       Triple
         (inv (⟨pref, cur::suff, h.symm⟩, b))
@@ -1330,8 +1307,8 @@ theorem Spec.forIn_rii {α β : Type u} {m : Type u → Type v} {l : Type u} {e 
 
 open Std Std.Iterators in
 @[lspec]
-theorem Spec.forIn_slice {δ : Type u} {m : Type u → Type w} {l : Type u} {e : Type u}
-    [Monad m] [AssertionLang l] [ExceptAssertionLang e] [WPMonad m l e] [LawfulMonad m]
+theorem Spec.forIn_slice {δ : Type u} {m : Type u → Type w} {Pred : Type u} {EPred : Type u}
+    [Monad m] [Assertion Pred] [Assertion EPred] [WP m Pred EPred] [LawfulMonad m]
     {γ : Type u'} {α β : Type u}
     [ToIterator (Slice γ) Id α β]
     [Iterator α Id β]
@@ -1340,8 +1317,8 @@ theorem Spec.forIn_slice {δ : Type u} {m : Type u → Type w} {l : Type u} {e :
     [Finite α Id]
     {init : δ} {f : β → δ → m (ForInStep δ)}
     {xs : Slice γ}
-    (inv : Invariant xs.toList δ l)
-    (eInv : e)
+    (inv : Invariant xs.toList δ Pred)
+    (eInv : EPred)
     (step : ∀ pref cur suff (h : xs.toList = pref ++ cur :: suff) b,
       Triple
         (inv (⟨pref, cur::suff, h.symm⟩, b))
@@ -1359,13 +1336,13 @@ section Iterators
 open Std Std.Iterators
 
 @[lspec]
-theorem Spec.forIn_iter {α β γ : Type u} {m : Type u → Type w} {l : Type u} {e : Type u}
-    [Monad m] [AssertionLang l] [ExceptAssertionLang e] [WPMonad m l e] [LawfulMonad m]
+theorem Spec.forIn_iter {α β γ : Type u} {m : Type u → Type w} {Pred : Type u} {EPred : Type u}
+    [Monad m] [Assertion Pred] [Assertion EPred] [WP m Pred EPred] [LawfulMonad m]
     [Iterator α Id β] [Finite α Id] [IteratorLoop α Id m] [LawfulIteratorLoop α Id m]
     {init : γ} {f : β → γ → m (ForInStep γ)}
     {it : Iter (α := α) β}
-    (inv : Invariant it.toList γ l)
-    (eInv : e)
+    (inv : Invariant it.toList γ Pred)
+    (eInv : EPred)
     (step : ∀ pref cur suff (h : it.toList = pref ++ cur :: suff) b,
       Triple
         (inv (⟨pref, cur::suff, h.symm⟩, b))
@@ -1380,13 +1357,13 @@ theorem Spec.forIn_iter {α β γ : Type u} {m : Type u → Type w} {l : Type u}
   exact Spec.forIn_list inv eInv step
 
 @[lspec]
-theorem Spec.forIn_iterM_id {α β γ : Type u} {m : Type u → Type w} {l : Type u} {e : Type u}
-    [Monad m] [AssertionLang l] [ExceptAssertionLang e] [WPMonad m l e] [LawfulMonad m]
+theorem Spec.forIn_iterM_id {α β γ : Type u} {m : Type u → Type w} {Pred : Type u} {EPred : Type u}
+    [Monad m] [Assertion Pred] [Assertion EPred] [WP m Pred EPred] [LawfulMonad m]
     [Iterator α Id β] [Finite α Id] [IteratorLoop α Id m] [LawfulIteratorLoop α Id m]
     {init : γ} {f : β → γ → m (ForInStep γ)}
     {it : IterM (α := α) Id β}
-    (inv : Invariant it.toList.run γ l)
-    (eInv : e)
+    (inv : Invariant it.toList.run γ Pred)
+    (eInv : EPred)
     (step : ∀ pref cur suff (h : it.toList.run = pref ++ cur :: suff) b,
       Triple
         (inv (⟨pref, cur::suff, h.symm⟩, b))
@@ -1403,13 +1380,13 @@ theorem Spec.forIn_iterM_id {α β γ : Type u} {m : Type u → Type w} {l : Typ
   exact Spec.forIn_list inv eInv step
 
 @[lspec]
-theorem Spec.foldM_iter {α β γ : Type u} {m : Type u → Type w} {l : Type u} {e : Type u}
-    [Monad m] [AssertionLang l] [ExceptAssertionLang e] [WPMonad m l e] [LawfulMonad m]
+theorem Spec.foldM_iter {α β γ : Type u} {m : Type u → Type w} {Pred : Type u} {EPred : Type u}
+    [Monad m] [Assertion Pred] [Assertion EPred] [WP m Pred EPred] [LawfulMonad m]
     [Iterator α Id β] [Finite α Id] [IteratorLoop α Id m] [LawfulIteratorLoop α Id m]
     {it : Iter (α := α) β}
     {init : γ} {f : γ → β → m γ}
-    (inv : Invariant it.toList γ l)
-    (eInv : e)
+    (inv : Invariant it.toList γ Pred)
+    (eInv : EPred)
     (step : ∀ pref cur suff (h : it.toList = pref ++ cur :: suff) b,
       Triple
         (inv (⟨pref, cur::suff, h.symm⟩, b))
@@ -1422,13 +1399,13 @@ theorem Spec.foldM_iter {α β γ : Type u} {m : Type u → Type w} {l : Type u}
   exact Spec.foldlM_list inv eInv step
 
 @[lspec]
-theorem Spec.foldM_iterM_id {α β γ : Type u} {m : Type u → Type w} {l : Type u} {e : Type u}
-    [Monad m] [AssertionLang l] [ExceptAssertionLang e] [WPMonad m l e] [LawfulMonad m]
+theorem Spec.foldM_iterM_id {α β γ : Type u} {m : Type u → Type w} {Pred : Type u} {EPred : Type u}
+    [Monad m] [Assertion Pred] [Assertion EPred] [WP m Pred EPred] [LawfulMonad m]
     [Iterator α Id β] [Finite α Id] [IteratorLoop α Id m] [LawfulIteratorLoop α Id m]
     {it : IterM (α := α) Id β}
     {init : γ} {f : γ → β → m γ}
-    (inv : Invariant it.toList.run γ l)
-    (eInv : e)
+    (inv : Invariant it.toList.run γ Pred)
+    (eInv : EPred)
     (step : ∀ pref cur suff (h : it.toList.run = pref ++ cur :: suff) b,
       Triple
         (inv (⟨pref, cur::suff, h.symm⟩, b))
@@ -1443,13 +1420,13 @@ theorem Spec.foldM_iterM_id {α β γ : Type u} {m : Type u → Type w} {l : Typ
 @[lspec]
 theorem Spec.IterM.forIn_filterMapWithPostcondition {α β β₂ γ : Type w}
     {m : Type w → Type w'} {n : Type w → Type w''} {o : Type w → Type w'''}
-    {l : Type w} {e : Type w}
-    [Monad m] [LawfulMonad m] [Monad n] [LawfulMonad n] [Monad o] [LawfulMonad o] [AssertionLang l] [ExceptAssertionLang e] [WPMonad o l e]
+    {Pred : Type w} {EPred : Type w}
+    [Monad m] [LawfulMonad m] [Monad n] [LawfulMonad n] [Monad o] [LawfulMonad o] [Assertion Pred] [Assertion EPred] [WP o Pred EPred]
     [MonadLiftT m n] [LawfulMonadLiftT m n] [MonadLiftT n o] [LawfulMonadLiftT n o]
     [Iterator α m β] [Finite α m]
     [IteratorLoop α m o] [LawfulIteratorLoop α m o]
     {it : IterM (α := α) m β} {f : β → PostconditionT n (Option β₂)} {init : γ}
-    {g : β₂ → γ → o (ForInStep γ)} {P : l} {Q : γ → l} {eQ : e}
+    {g : β₂ → γ → o (ForInStep γ)} {P : Pred} {Q : γ → Pred} {eQ : EPred}
     (h :
         haveI : MonadLift n o := ⟨monadLift⟩
         Triple P (forIn (m := o) it init (fun out acc => do
@@ -1462,14 +1439,14 @@ theorem Spec.IterM.forIn_filterMapWithPostcondition {α β β₂ γ : Type w}
 @[lspec]
 theorem Spec.IterM.forIn_filterMapM {α β β₂ γ : Type w}
     {m : Type w → Type w'} {n : Type w → Type w''} {o : Type w → Type w'''}
-    {l : Type w} {e : Type w}
-    [Monad m] [LawfulMonad m] [Monad n] [LawfulMonad n] [Monad o] [LawfulMonad o] [AssertionLang l] [ExceptAssertionLang e] [WPMonad o l e]
+    {Pred : Type w} {EPred : Type w}
+    [Monad m] [LawfulMonad m] [Monad n] [LawfulMonad n] [Monad o] [LawfulMonad o] [Assertion Pred] [Assertion EPred] [WP o Pred EPred]
     [MonadAttach n] [WeaklyLawfulMonadAttach n]
     [MonadLiftT m n] [LawfulMonadLiftT m n] [MonadLiftT n o] [LawfulMonadLiftT n o]
     [Iterator α m β] [Finite α m]
     [IteratorLoop α m o] [LawfulIteratorLoop α m o]
     {it : IterM (α := α) m β} {f : β → n (Option β₂)} {init : γ} {g : β₂ → γ → o (ForInStep γ)}
-    {P : l} {Q : γ → l} {eQ : e}
+    {P : Pred} {Q : γ → Pred} {eQ : EPred}
     (h :
         haveI : MonadLift n o := ⟨monadLift⟩
         Triple P (forIn (m := o) it init (fun out acc => do
@@ -1482,13 +1459,13 @@ theorem Spec.IterM.forIn_filterMapM {α β β₂ γ : Type w}
 @[lspec]
 theorem Spec.IterM.forIn_filterMap {α β β₂ γ : Type w}
     {m : Type w → Type w'} {n : Type w → Type w''}
-    {l : Type w} {e : Type w}
-    [Monad m] [LawfulMonad m] [Monad n] [LawfulMonad n] [AssertionLang l] [ExceptAssertionLang e] [WPMonad n l e]
+    {Pred : Type w} {EPred : Type w}
+    [Monad m] [LawfulMonad m] [Monad n] [LawfulMonad n] [Assertion Pred] [Assertion EPred] [WP n Pred EPred]
     [MonadLiftT m n] [LawfulMonadLiftT m n]
     [Iterator α m β] [Finite α m]
     [IteratorLoop α m n] [LawfulIteratorLoop α m n]
     {it : IterM (α := α) m β} {f : β → Option β₂} {init : γ} {g : β₂ → γ → n (ForInStep γ)}
-    {P : l} {Q : γ → l} {eQ : e}
+    {P : Pred} {Q : γ → Pred} {eQ : EPred}
     (h : Triple P (forIn it init (fun out acc => do
           match f out with
           | some c => g c acc
@@ -1499,13 +1476,13 @@ theorem Spec.IterM.forIn_filterMap {α β β₂ γ : Type w}
 @[lspec]
 theorem Spec.IterM.forIn_mapWithPostcondition {α β β₂ γ : Type w}
     {m : Type w → Type w'} {n : Type w → Type w''} {o : Type w → Type w'''}
-    {l : Type w} {e : Type w}
-    [Monad m] [LawfulMonad m] [Monad n] [LawfulMonad n] [Monad o] [LawfulMonad o] [AssertionLang l] [ExceptAssertionLang e] [WPMonad o l e]
+    {Pred : Type w} {EPred : Type w}
+    [Monad m] [LawfulMonad m] [Monad n] [LawfulMonad n] [Monad o] [LawfulMonad o] [Assertion Pred] [Assertion EPred] [WP o Pred EPred]
     [MonadLiftT m n] [LawfulMonadLiftT m n] [MonadLiftT n o] [LawfulMonadLiftT n o]
     [Iterator α m β] [Finite α m]
     [IteratorLoop α m o] [LawfulIteratorLoop α m o]
     {it : IterM (α := α) m β} {f : β → PostconditionT n β₂} {init : γ}
-    {g : β₂ → γ → o (ForInStep γ)} {P : l} {Q : γ → l} {eQ : e}
+    {g : β₂ → γ → o (ForInStep γ)} {P : Pred} {Q : γ → Pred} {eQ : EPred}
     (h :
         haveI : MonadLift n o := ⟨monadLift⟩
         Triple P (forIn (m := o) it init (fun out acc => do g (← (f out).run) acc)) Q eQ) :
@@ -1515,14 +1492,14 @@ theorem Spec.IterM.forIn_mapWithPostcondition {α β β₂ γ : Type w}
 @[lspec]
 theorem Spec.IterM.forIn_mapM {α β β₂ γ : Type w}
     {m : Type w → Type w'} {n : Type w → Type w''} {o : Type w → Type w'''}
-    {l : Type w} {e : Type w}
-    [Monad m] [LawfulMonad m] [Monad n] [LawfulMonad n] [Monad o] [LawfulMonad o] [AssertionLang l] [ExceptAssertionLang e] [WPMonad o l e]
+    {Pred : Type w} {EPred : Type w}
+    [Monad m] [LawfulMonad m] [Monad n] [LawfulMonad n] [Monad o] [LawfulMonad o] [Assertion Pred] [Assertion EPred] [WP o Pred EPred]
     [MonadAttach n] [WeaklyLawfulMonadAttach n]
     [MonadLiftT m n] [LawfulMonadLiftT m n] [MonadLiftT n o] [LawfulMonadLiftT n o]
     [Iterator α m β] [Finite α m]
     [IteratorLoop α m o] [LawfulIteratorLoop α m o]
     {it : IterM (α := α) m β} {f : β → n β₂} {init : γ} {g : β₂ → γ → o (ForInStep γ)}
-    {P : l} {Q : γ → l} {eQ : e}
+    {P : Pred} {Q : γ → Pred} {eQ : EPred}
     (h :
         haveI : MonadLift n o := ⟨monadLift⟩
         Triple P (forIn (m := o) it init (fun out acc => do g (← f out) acc)) Q eQ) :
@@ -1532,12 +1509,12 @@ theorem Spec.IterM.forIn_mapM {α β β₂ γ : Type w}
 @[lspec]
 theorem Spec.IterM.forIn_map {α β β₂ γ : Type w}
     {m : Type w → Type w'} {n : Type w → Type w''}
-    {l : Type w} {e : Type w}
-    [Monad m] [LawfulMonad m] [Monad n] [LawfulMonad n] [AssertionLang l] [ExceptAssertionLang e] [WPMonad n l e]
+    {Pred : Type w} {EPred : Type w}
+    [Monad m] [LawfulMonad m] [Monad n] [LawfulMonad n] [Assertion Pred] [Assertion EPred] [WP n Pred EPred]
     [MonadLiftT m n] [LawfulMonadLiftT m n]
     [Iterator α m β] [Finite α m] [IteratorLoop α m n] [LawfulIteratorLoop α m n]
     {it : IterM (α := α) m β} {f : β → β₂} {init : γ} {g : β₂ → γ → n (ForInStep γ)}
-    {P : l} {Q : γ → l} {eQ : e}
+    {P : Pred} {Q : γ → Pred} {eQ : EPred}
     (h : Triple P (forIn it init (fun out acc => do g (f out) acc)) Q eQ) :
     Triple P (forIn (it.map f) init g) Q eQ := by
   rwa [Std.IterM.forIn_map]
@@ -1545,13 +1522,13 @@ theorem Spec.IterM.forIn_map {α β β₂ γ : Type w}
 @[lspec]
 theorem Spec.IterM.forIn_filterWithPostcondition {α β γ : Type w}
     {m : Type w → Type w'} {n : Type w → Type w''} {o : Type w → Type w'''}
-    {l : Type w} {e : Type w}
-    [Monad m] [LawfulMonad m] [Monad n] [LawfulMonad n] [Monad o] [LawfulMonad o] [AssertionLang l] [ExceptAssertionLang e] [WPMonad o l e]
+    {Pred : Type w} {EPred : Type w}
+    [Monad m] [LawfulMonad m] [Monad n] [LawfulMonad n] [Monad o] [LawfulMonad o] [Assertion Pred] [Assertion EPred] [WP o Pred EPred]
     [MonadLiftT m n] [LawfulMonadLiftT m n] [MonadLiftT n o] [LawfulMonadLiftT n o]
     [Iterator α m β] [Finite α m]
     [IteratorLoop α m o] [LawfulIteratorLoop α m o]
     {it : IterM (α := α) m β} {f : β → PostconditionT n (ULift Bool)} {init : γ}
-    {g : β → γ → o (ForInStep γ)} {P : l} {Q : γ → l} {eQ : e}
+    {g : β → γ → o (ForInStep γ)} {P : Pred} {Q : γ → Pred} {eQ : EPred}
     (h :
         haveI : MonadLift n o := ⟨monadLift⟩
         Triple P (forIn (m := o) it init (fun out acc => do if (← (f out).run).down then g out acc else return .yield acc)) Q eQ) :
@@ -1561,14 +1538,14 @@ theorem Spec.IterM.forIn_filterWithPostcondition {α β γ : Type w}
 @[lspec]
 theorem Spec.IterM.forIn_filterM {α β γ : Type w}
     {m : Type w → Type w'} {n : Type w → Type w''} {o : Type w → Type w'''}
-    {l : Type w} {e : Type w}
-    [Monad m] [LawfulMonad m] [Monad n] [LawfulMonad n] [Monad o] [LawfulMonad o] [AssertionLang l] [ExceptAssertionLang e] [WPMonad o l e]
+    {Pred : Type w} {EPred : Type w}
+    [Monad m] [LawfulMonad m] [Monad n] [LawfulMonad n] [Monad o] [LawfulMonad o] [Assertion Pred] [Assertion EPred] [WP o Pred EPred]
     [MonadAttach n] [WeaklyLawfulMonadAttach n]
     [MonadLiftT m n] [LawfulMonadLiftT m n] [MonadLiftT n o] [LawfulMonadLiftT n o]
     [Iterator α m β] [Finite α m]
     [IteratorLoop α m o] [LawfulIteratorLoop α m o]
     {it : IterM (α := α) m β} {f : β → n (ULift Bool)} {init : γ} {g : β → γ → o (ForInStep γ)}
-    {P : l} {Q : γ → l} {eQ : e}
+    {P : Pred} {Q : γ → Pred} {eQ : EPred}
     (h :
         haveI : MonadLift n o := ⟨monadLift⟩
         Triple P (forIn (m := o) it init (fun out acc => do if (← f out).down then g out acc else return .yield acc)) Q eQ) :
@@ -1578,12 +1555,12 @@ theorem Spec.IterM.forIn_filterM {α β γ : Type w}
 @[lspec]
 theorem Spec.IterM.forIn_filter {α β γ : Type w}
     {m : Type w → Type w'} {n : Type w → Type w''}
-    {l : Type w} {e : Type w}
-    [Monad m] [LawfulMonad m] [Monad n] [LawfulMonad n] [AssertionLang l] [ExceptAssertionLang e] [WPMonad n l e]
+    {Pred : Type w} {EPred : Type w}
+    [Monad m] [LawfulMonad m] [Monad n] [LawfulMonad n] [Assertion Pred] [Assertion EPred] [WP n Pred EPred]
     [MonadLiftT m n] [LawfulMonadLiftT m n]
     [Iterator α m β] [Finite α m] [IteratorLoop α m n] [LawfulIteratorLoop α m n]
     {it : IterM (α := α) m β} {f : β → Bool} {init : γ} {g : β → γ → n (ForInStep γ)}
-    {P : l} {Q : γ → l} {eQ : e}
+    {P : Pred} {Q : γ → Pred} {eQ : EPred}
     (h : Triple P (forIn (m := n) it init (fun out acc => do if f out then g out acc else return .yield acc)) Q eQ) :
     Triple P (forIn (it.filter f) init g) Q eQ := by
   rwa [Std.IterM.forIn_filter]
@@ -1591,14 +1568,14 @@ theorem Spec.IterM.forIn_filter {α β γ : Type w}
 @[lspec]
 theorem Spec.IterM.foldM_filterMapWithPostcondition {α β γ δ : Type w}
     {m : Type w → Type w'} {n : Type w → Type w''} {o : Type w → Type w'''}
-    {l : Type w} {e : Type w}
+    {Pred : Type w} {EPred : Type w}
     [Iterator α m β] [Finite α m]
-    [Monad m] [Monad n] [Monad o] [LawfulMonad m] [LawfulMonad n] [LawfulMonad o] [AssertionLang l] [ExceptAssertionLang e] [WPMonad o l e]
+    [Monad m] [Monad n] [Monad o] [LawfulMonad m] [LawfulMonad n] [LawfulMonad o] [Assertion Pred] [Assertion EPred] [WP o Pred EPred]
     [IteratorLoop α m n] [IteratorLoop α m o]
     [LawfulIteratorLoop α m n] [LawfulIteratorLoop α m o]
     [MonadLiftT m n] [MonadLiftT n o] [LawfulMonadLiftT m n] [LawfulMonadLiftT n o]
     {f : β → PostconditionT n (Option γ)} {g : δ → γ → o δ} {init : δ} {it : IterM (α := α) m β}
-    {P : l} {Q : δ → l} {eQ : e}
+    {P : Pred} {Q : δ → Pred} {eQ : EPred}
     (h :
         haveI : MonadLift n o := ⟨MonadLiftT.monadLift⟩
         Triple P (it.foldM (n := o) (init := init) (fun d b => do
@@ -1610,16 +1587,16 @@ theorem Spec.IterM.foldM_filterMapWithPostcondition {α β γ δ : Type w}
 @[lspec]
 theorem Spec.IterM.foldM_filterMapM {α β γ δ : Type w}
     {m : Type w → Type w'} {n : Type w → Type w''} {o : Type w → Type w'''}
-    {l : Type w} {e : Type w}
+    {Pred : Type w} {EPred : Type w}
     [Iterator α m β] [Finite α m]
     [Monad m] [LawfulMonad m]
     [Monad n] [MonadAttach n] [LawfulMonad n] [WeaklyLawfulMonadAttach n]
-    [Monad o] [LawfulMonad o] [AssertionLang l] [ExceptAssertionLang e] [WPMonad o l e]
+    [Monad o] [LawfulMonad o] [Assertion Pred] [Assertion EPred] [WP o Pred EPred]
     [IteratorLoop α m n] [IteratorLoop α m o]
     [LawfulIteratorLoop α m n] [LawfulIteratorLoop α m o]
     [MonadLiftT m n] [MonadLiftT n o] [LawfulMonadLiftT m n] [LawfulMonadLiftT n o]
     {f : β → n (Option γ)} {g : δ → γ → o δ} {init : δ} {it : IterM (α := α) m β}
-    {P : l} {Q : δ → l} {eQ : e}
+    {P : Pred} {Q : δ → Pred} {eQ : EPred}
     (h :
         haveI : MonadLift n o := ⟨MonadLiftT.monadLift⟩
         Triple P (it.foldM (n := o) (init := init) (fun d b => do
@@ -1631,14 +1608,14 @@ theorem Spec.IterM.foldM_filterMapM {α β γ δ : Type w}
 @[lspec]
 theorem Spec.IterM.foldM_mapWithPostcondition {α β γ δ : Type w}
     {m : Type w → Type w'} {n : Type w → Type w''} {o : Type w → Type w'''}
-    {l : Type w} {e : Type w}
+    {Pred : Type w} {EPred : Type w}
     [Iterator α m β] [Finite α m]
-    [Monad m] [Monad n] [Monad o] [LawfulMonad m] [LawfulMonad n] [LawfulMonad o] [AssertionLang l] [ExceptAssertionLang e] [WPMonad o l e]
+    [Monad m] [Monad n] [Monad o] [LawfulMonad m] [LawfulMonad n] [LawfulMonad o] [Assertion Pred] [Assertion EPred] [WP o Pred EPred]
     [IteratorLoop α m n] [IteratorLoop α m o]
     [LawfulIteratorLoop α m n] [LawfulIteratorLoop α m o]
     [MonadLiftT m n] [MonadLiftT n o] [LawfulMonadLiftT m n] [LawfulMonadLiftT n o]
     {f : β → PostconditionT n γ} {g : δ → γ → o δ} {init : δ} {it : IterM (α := α) m β}
-    {P : l} {Q : δ → l} {eQ : e}
+    {P : Pred} {Q : δ → Pred} {eQ : EPred}
     (h :
         haveI : MonadLift n o := ⟨MonadLiftT.monadLift⟩
         Triple P (it.foldM (n := o) (init := init) (fun d b => do let c ← (f b).run; g d c)) Q eQ) :
@@ -1648,16 +1625,16 @@ theorem Spec.IterM.foldM_mapWithPostcondition {α β γ δ : Type w}
 @[lspec]
 theorem Spec.IterM.foldM_mapM {α β γ δ : Type w}
     {m : Type w → Type w'} {n : Type w → Type w''} {o : Type w → Type w'''}
-    {l : Type w} {e : Type w}
+    {Pred : Type w} {EPred : Type w}
     [Iterator α m β] [Finite α m]
     [Monad m] [LawfulMonad m]
     [Monad n] [MonadAttach n] [LawfulMonad n] [WeaklyLawfulMonadAttach n]
-    [Monad o] [LawfulMonad o] [AssertionLang l] [ExceptAssertionLang e] [WPMonad o l e]
+    [Monad o] [LawfulMonad o] [Assertion Pred] [Assertion EPred] [WP o Pred EPred]
     [IteratorLoop α m n] [IteratorLoop α m o]
     [LawfulIteratorLoop α m n] [LawfulIteratorLoop α m o]
     [MonadLiftT m n] [MonadLiftT n o] [LawfulMonadLiftT m n] [LawfulMonadLiftT n o]
     {f : β → n γ} {g : δ → γ → o δ} {init : δ} {it : IterM (α := α) m β}
-    {P : l} {Q : δ → l} {eQ : e}
+    {P : Pred} {Q : δ → Pred} {eQ : EPred}
     (h :
         haveI : MonadLift n o := ⟨MonadLiftT.monadLift⟩
         Triple P (it.foldM (n := o) (init := init) (fun d b => do let c ← f b; g d c)) Q eQ) :
@@ -1667,14 +1644,14 @@ theorem Spec.IterM.foldM_mapM {α β γ δ : Type w}
 @[lspec]
 theorem Spec.IterM.foldM_filterWithPostcondition {α β δ : Type w}
     {m : Type w → Type w'} {n : Type w → Type w''} {o : Type w → Type w'''}
-    {l : Type w} {e : Type w}
+    {Pred : Type w} {EPred : Type w}
     [Iterator α m β] [Finite α m]
-    [Monad m] [Monad n] [Monad o] [LawfulMonad m] [LawfulMonad n] [LawfulMonad o] [AssertionLang l] [ExceptAssertionLang e] [WPMonad o l e]
+    [Monad m] [Monad n] [Monad o] [LawfulMonad m] [LawfulMonad n] [LawfulMonad o] [Assertion Pred] [Assertion EPred] [WP o Pred EPred]
     [IteratorLoop α m n] [IteratorLoop α m o]
     [LawfulIteratorLoop α m n] [LawfulIteratorLoop α m o]
     [MonadLiftT m n] [MonadLiftT n o] [LawfulMonadLiftT m n] [LawfulMonadLiftT n o]
     {f : β → PostconditionT n (ULift Bool)} {g : δ → β → o δ} {init : δ} {it : IterM (α := α) m β}
-    {P : l} {Q : δ → l} {eQ : e}
+    {P : Pred} {Q : δ → Pred} {eQ : EPred}
     (h :
         haveI : MonadLift n o := ⟨MonadLiftT.monadLift⟩
         Triple P (it.foldM (n := o) (init := init) (fun d b => do if (← (f b).run).down then g d b else Pure.pure d)) Q eQ) :
@@ -1684,16 +1661,16 @@ theorem Spec.IterM.foldM_filterWithPostcondition {α β δ : Type w}
 @[lspec]
 theorem Spec.IterM.foldM_filterM {α β δ : Type w}
     {m : Type w → Type w'} {n : Type w → Type w''} {o : Type w → Type w'''}
-    {l : Type w} {e : Type w}
+    {Pred : Type w} {EPred : Type w}
     [Iterator α m β] [Finite α m]
     [Monad m] [LawfulMonad m]
     [Monad n] [MonadAttach n] [LawfulMonad n] [WeaklyLawfulMonadAttach n]
-    [Monad o] [LawfulMonad o] [AssertionLang l] [ExceptAssertionLang e] [WPMonad o l e]
+    [Monad o] [LawfulMonad o] [Assertion Pred] [Assertion EPred] [WP o Pred EPred]
     [IteratorLoop α m n] [IteratorLoop α m o]
     [LawfulIteratorLoop α m n] [LawfulIteratorLoop α m o]
     [MonadLiftT m n] [MonadLiftT n o] [LawfulMonadLiftT m n] [LawfulMonadLiftT n o]
     {f : β → n (ULift Bool)} {g : δ → β → o δ} {init : δ} {it : IterM (α := α) m β}
-    {P : l} {Q : δ → l} {eQ : e}
+    {P : Pred} {Q : δ → Pred} {eQ : EPred}
     (h :
         haveI : MonadLift n o := ⟨MonadLiftT.monadLift⟩
         Triple P (it.foldM (n := o) (init := init) (fun d b => do if (← f b).down then g d b else Pure.pure d)) Q eQ) :
@@ -1703,13 +1680,13 @@ theorem Spec.IterM.foldM_filterM {α β δ : Type w}
 @[lspec]
 theorem Spec.IterM.foldM_filterMap {α β γ δ : Type w}
     {m : Type w → Type w'} {n : Type w → Type w''}
-    {l : Type w} {e : Type w}
-    [Iterator α m β] [Finite α m] [Monad m] [Monad n] [LawfulMonad m] [LawfulMonad n] [AssertionLang l] [ExceptAssertionLang e] [WPMonad n l e]
+    {Pred : Type w} {EPred : Type w}
+    [Iterator α m β] [Finite α m] [Monad m] [Monad n] [LawfulMonad m] [LawfulMonad n] [Assertion Pred] [Assertion EPred] [WP n Pred EPred]
     [IteratorLoop α m n]
     [LawfulIteratorLoop α m n]
     [MonadLiftT m n] [LawfulMonadLiftT m n]
     {f : β → Option γ} {g : δ → γ → n δ} {init : δ} {it : IterM (α := α) m β}
-    {P : l} {Q : δ → l} {eQ : e}
+    {P : Pred} {Q : δ → Pred} {eQ : EPred}
     (h : Triple P (it.foldM (n := n) (init := init) (fun d b => do
           let some c := f b | Pure.pure d
           g d c)) Q eQ) :
@@ -1719,12 +1696,12 @@ theorem Spec.IterM.foldM_filterMap {α β γ δ : Type w}
 @[lspec]
 theorem Spec.IterM.foldM_map {α β γ δ : Type w}
     {m : Type w → Type w'} {n : Type w → Type w''}
-    {l : Type w} {e : Type w}
-    [Iterator α m β] [Finite α m] [Monad m] [Monad n] [LawfulMonad m] [LawfulMonad n] [AssertionLang l] [ExceptAssertionLang e] [WPMonad n l e]
+    {Pred : Type w} {EPred : Type w}
+    [Iterator α m β] [Finite α m] [Monad m] [Monad n] [LawfulMonad m] [LawfulMonad n] [Assertion Pred] [Assertion EPred] [WP n Pred EPred]
     [IteratorLoop α m n] [LawfulIteratorLoop α m n]
     [MonadLiftT m n] [LawfulMonadLiftT m n]
     {f : β → γ} {g : δ → γ → n δ} {init : δ} {it : IterM (α := α) m β}
-    {P : l} {Q : δ → l} {eQ : e}
+    {P : Pred} {Q : δ → Pred} {eQ : EPred}
     (h : Triple P (it.foldM (init := init) (fun d b => do g d (f b))) Q eQ) :
     Triple P ((it.map f).foldM (init := init) g) Q eQ := by
   rwa [Std.IterM.foldM_map]
@@ -1732,13 +1709,13 @@ theorem Spec.IterM.foldM_map {α β γ δ : Type w}
 @[lspec]
 theorem Spec.IterM.foldM_filter {α β δ : Type w}
     {m : Type w → Type w'} {n : Type w → Type w''}
-    {l : Type w} {e : Type w}
-    [Iterator α m β] [Finite α m] [Monad m] [Monad n] [LawfulMonad m] [LawfulMonad n] [AssertionLang l] [ExceptAssertionLang e] [WPMonad n l e]
+    {Pred : Type w} {EPred : Type w}
+    [Iterator α m β] [Finite α m] [Monad m] [Monad n] [LawfulMonad m] [LawfulMonad n] [Assertion Pred] [Assertion EPred] [WP n Pred EPred]
     [IteratorLoop α m n]
     [LawfulIteratorLoop α m n]
     [MonadLiftT m n] [LawfulMonadLiftT m n]
     {f : β → Bool} {g : δ → β → n δ} {init : δ} {it : IterM (α := α) m β}
-    {P : l} {Q : δ → l} {eQ : e}
+    {P : Pred} {Q : δ → Pred} {eQ : EPred}
     (h : Triple P (it.foldM (init := init) (fun d b => if f b then g d b else Pure.pure d)) Q eQ) :
     Triple P ((it.filter f).foldM (init := init) g) Q eQ := by
   rwa [Std.IterM.foldM_filter]
@@ -1746,14 +1723,14 @@ theorem Spec.IterM.foldM_filter {α β δ : Type w}
 @[lspec]
 theorem Spec.IterM.fold_filterMapWithPostcondition {α β γ δ : Type w}
     {m : Type w → Type w'} {n : Type w → Type w''}
-    {l : Type w} {e : Type w}
+    {Pred : Type w} {EPred : Type w}
     [Iterator α m β] [Finite α m]
     [Monad m] [LawfulMonad m]
-    [Monad n] [LawfulMonad n] [AssertionLang l] [ExceptAssertionLang e] [WPMonad n l e]
+    [Monad n] [LawfulMonad n] [Assertion Pred] [Assertion EPred] [WP n Pred EPred]
     [IteratorLoop α m n] [LawfulIteratorLoop α m n]
     [MonadLiftT m n] [LawfulMonadLiftT m n]
     {f : β → PostconditionT n (Option γ)} {g : δ → γ → δ} {init : δ} {it : IterM (α := α) m β}
-    {P : l} {Q : δ → l} {eQ : e}
+    {P : Pred} {Q : δ → Pred} {eQ : EPred}
     (h : Triple P (it.foldM (n := n) (init := init) (fun d b => do
           let some c ← (f b).run | Pure.pure d
           return g d c)) Q eQ) :
@@ -1763,14 +1740,14 @@ theorem Spec.IterM.fold_filterMapWithPostcondition {α β γ δ : Type w}
 @[lspec]
 theorem Spec.IterM.fold_filterMapM {α β γ δ : Type w}
     {m : Type w → Type w'} {n : Type w → Type w''}
-    {l : Type w} {e : Type w}
+    {Pred : Type w} {EPred : Type w}
     [Iterator α m β] [Finite α m]
     [Monad m] [LawfulMonad m]
-    [Monad n] [MonadAttach n] [LawfulMonad n] [WeaklyLawfulMonadAttach n] [AssertionLang l] [ExceptAssertionLang e] [WPMonad n l e]
+    [Monad n] [MonadAttach n] [LawfulMonad n] [WeaklyLawfulMonadAttach n] [Assertion Pred] [Assertion EPred] [WP n Pred EPred]
     [IteratorLoop α m n] [LawfulIteratorLoop α m n]
     [MonadLiftT m n] [LawfulMonadLiftT m n]
     {f : β → n (Option γ)} {g : δ → γ → δ} {init : δ} {it : IterM (α := α) m β}
-    {P : l} {Q : δ → l} {eQ : e}
+    {P : Pred} {Q : δ → Pred} {eQ : EPred}
     (h : Triple P (it.foldM (init := init) (fun d b => do
           let some c ← f b | Pure.pure d
           return g d c)) Q eQ) :
@@ -1780,14 +1757,14 @@ theorem Spec.IterM.fold_filterMapM {α β γ δ : Type w}
 @[lspec]
 theorem Spec.IterM.fold_mapWithPostcondition {α β γ δ : Type w}
     {m : Type w → Type w'} {n : Type w → Type w''}
-    {l : Type w} {e : Type w}
+    {Pred : Type w} {EPred : Type w}
     [Iterator α m β] [Finite α m]
     [Monad m] [LawfulMonad m]
-    [Monad n] [LawfulMonad n] [AssertionLang l] [ExceptAssertionLang e] [WPMonad n l e]
+    [Monad n] [LawfulMonad n] [Assertion Pred] [Assertion EPred] [WP n Pred EPred]
     [IteratorLoop α m n] [LawfulIteratorLoop α m n]
     [MonadLiftT m n] [LawfulMonadLiftT m n]
     {f : β → PostconditionT n γ} {g : δ → γ → δ} {init : δ} {it : IterM (α := α) m β}
-    {P : l} {Q : δ → l} {eQ : e}
+    {P : Pred} {Q : δ → Pred} {eQ : EPred}
     (h : Triple P (it.foldM (init := init) (fun d b => do let c ← (f b).run; return g d c)) Q eQ) :
     Triple P ((it.mapWithPostcondition f).fold (init := init) g) Q eQ := by
   rwa [Std.IterM.fold_mapWithPostcondition]
@@ -1795,14 +1772,14 @@ theorem Spec.IterM.fold_mapWithPostcondition {α β γ δ : Type w}
 @[lspec]
 theorem Spec.IterM.fold_mapM {α β γ δ : Type w}
     {m : Type w → Type w'} {n : Type w → Type w''}
-    {l : Type w} {e : Type w}
+    {Pred : Type w} {EPred : Type w}
     [Iterator α m β] [Finite α m]
     [Monad m] [LawfulMonad m]
-    [Monad n] [MonadAttach n] [LawfulMonad n] [WeaklyLawfulMonadAttach n] [AssertionLang l] [ExceptAssertionLang e] [WPMonad n l e]
+    [Monad n] [MonadAttach n] [LawfulMonad n] [WeaklyLawfulMonadAttach n] [Assertion Pred] [Assertion EPred] [WP n Pred EPred]
     [IteratorLoop α m n] [LawfulIteratorLoop α m n]
     [MonadLiftT m n] [LawfulMonadLiftT m n]
     {f : β → n γ} {g : δ → γ → δ} {init : δ} {it : IterM (α := α) m β}
-    {P : l} {Q : δ → l} {eQ : e}
+    {P : Pred} {Q : δ → Pred} {eQ : EPred}
     (h : Triple P (it.foldM (init := init) (fun d b => do let c ← f b; return g d c)) Q eQ) :
     Triple P ((it.mapM f).fold (init := init) g) Q eQ := by
   rwa [Std.IterM.fold_mapM]
@@ -1810,14 +1787,14 @@ theorem Spec.IterM.fold_mapM {α β γ δ : Type w}
 @[lspec]
 theorem Spec.IterM.fold_filterWithPostcondition {α β δ : Type w}
     {m : Type w → Type w'} {n : Type w → Type w''}
-    {l : Type w} {e : Type w}
+    {Pred : Type w} {EPred : Type w}
     [Iterator α m β] [Finite α m]
     [Monad m] [LawfulMonad m]
-    [Monad n] [LawfulMonad n] [AssertionLang l] [ExceptAssertionLang e] [WPMonad n l e]
+    [Monad n] [LawfulMonad n] [Assertion Pred] [Assertion EPred] [WP n Pred EPred]
     [IteratorLoop α m n] [LawfulIteratorLoop α m n]
     [MonadLiftT m n] [LawfulMonadLiftT m n]
     {f : β → PostconditionT n (ULift Bool)} {g : δ → β → δ} {init : δ} {it : IterM (α := α) m β}
-    {P : l} {Q : δ → l} {eQ : e}
+    {P : Pred} {Q : δ → Pred} {eQ : EPred}
     (h : Triple P (it.foldM (init := init) (fun d b => return if (← (f b).run).down then g d b else d)) Q eQ) :
     Triple P ((it.filterWithPostcondition f).fold (init := init) g) Q eQ := by
   rwa [Std.IterM.fold_filterWithPostcondition]
@@ -1825,14 +1802,14 @@ theorem Spec.IterM.fold_filterWithPostcondition {α β δ : Type w}
 @[lspec]
 theorem Spec.IterM.fold_filterM {α β δ : Type w}
     {m : Type w → Type w'} {n : Type w → Type w''}
-    {l : Type w} {e : Type w}
+    {Pred : Type w} {EPred : Type w}
     [Iterator α m β] [Finite α m]
     [Monad m] [LawfulMonad m]
-    [Monad n] [MonadAttach n] [LawfulMonad n] [WeaklyLawfulMonadAttach n] [AssertionLang l] [ExceptAssertionLang e] [WPMonad n l e]
+    [Monad n] [MonadAttach n] [LawfulMonad n] [WeaklyLawfulMonadAttach n] [Assertion Pred] [Assertion EPred] [WP n Pred EPred]
     [IteratorLoop α m n] [LawfulIteratorLoop α m n]
     [MonadLiftT m n] [LawfulMonadLiftT m n]
     {f : β → n (ULift Bool)} {g : δ → β → δ} {init : δ} {it : IterM (α := α) m β}
-    {P : l} {Q : δ → l} {eQ : e}
+    {P : Pred} {Q : δ → Pred} {eQ : EPred}
     (h : Triple P (it.foldM (init := init) (fun d b => return if (← f b).down then g d b else d)) Q eQ) :
     Triple P ((it.filterM f).fold (init := init) g) Q eQ := by
   rwa [Std.IterM.fold_filterM]
@@ -1840,11 +1817,11 @@ theorem Spec.IterM.fold_filterM {α β δ : Type w}
 @[lspec]
 theorem Spec.IterM.fold_filterMap {α β γ δ : Type w}
     {m : Type w → Type w'}
-    {l : Type w} {e : Type w}
-    [Iterator α m β] [Finite α m] [Monad m] [LawfulMonad m] [AssertionLang l] [ExceptAssertionLang e] [WPMonad m l e]
+    {Pred : Type w} {EPred : Type w}
+    [Iterator α m β] [Finite α m] [Monad m] [LawfulMonad m] [Assertion Pred] [Assertion EPred] [WP m Pred EPred]
     [IteratorLoop α m m] [LawfulIteratorLoop α m m]
     {f : β → Option γ} {g : δ → γ → δ} {init : δ} {it : IterM (α := α) m β}
-    {P : l} {Q : δ → l} {eQ : e}
+    {P : Pred} {Q : δ → Pred} {eQ : EPred}
     (h : Triple P (it.fold (init := init) (fun d b =>
           match f b with
           | some c => g d c
@@ -1855,11 +1832,11 @@ theorem Spec.IterM.fold_filterMap {α β γ δ : Type w}
 @[lspec]
 theorem Spec.IterM.fold_map {α β γ δ : Type w}
     {m : Type w → Type w'}
-    {l : Type w} {e : Type w}
-    [Iterator α m β] [Finite α m] [Monad m] [LawfulMonad m] [AssertionLang l] [ExceptAssertionLang e] [WPMonad m l e]
+    {Pred : Type w} {EPred : Type w}
+    [Iterator α m β] [Finite α m] [Monad m] [LawfulMonad m] [Assertion Pred] [Assertion EPred] [WP m Pred EPred]
     [IteratorLoop α m m] [LawfulIteratorLoop α m m]
     {f : β → γ} {g : δ → γ → δ} {init : δ} {it : IterM (α := α) m β}
-    {P : l} {Q : δ → l} {eQ : e}
+    {P : Pred} {Q : δ → Pred} {eQ : EPred}
     (h : Triple P (it.fold (init := init) (fun d b => g d (f b))) Q eQ) :
     Triple P ((it.map f).fold (init := init) g) Q eQ := by
   rwa [Std.IterM.fold_map]
@@ -1867,11 +1844,11 @@ theorem Spec.IterM.fold_map {α β γ δ : Type w}
 @[lspec]
 theorem Spec.IterM.fold_filter {α β δ : Type w}
     {m : Type w → Type w'}
-    {l : Type w} {e : Type w}
-    [Iterator α m β] [Finite α m] [Monad m] [LawfulMonad m] [AssertionLang l] [ExceptAssertionLang e] [WPMonad m l e]
+    {Pred : Type w} {EPred : Type w}
+    [Iterator α m β] [Finite α m] [Monad m] [LawfulMonad m] [Assertion Pred] [Assertion EPred] [WP m Pred EPred]
     [IteratorLoop α m m] [LawfulIteratorLoop α m m]
     {f : β → Bool} {g : δ → β → δ} {init : δ} {it : IterM (α := α) m β}
-    {P : l} {Q : δ → l} {eQ : e}
+    {P : Pred} {Q : δ → Pred} {eQ : EPred}
     (h : Triple P (it.fold (init := init) (fun d b => if f b then g d b else d)) Q eQ) :
     Triple P ((it.filter f).fold (init := init) g) Q eQ := by
   rwa [Std.IterM.fold_filter]
@@ -1879,13 +1856,13 @@ theorem Spec.IterM.fold_filter {α β δ : Type w}
 @[lspec]
 theorem Spec.Iter.forIn_filterMapWithPostcondition {α β β₂ γ : Type w}
     {n : Type w → Type w'} {o : Type w → Type w''}
-    {l : Type w} {e : Type w}
+    {Pred : Type w} {EPred : Type w}
     [Iterator α Id β]
-    [Monad n] [LawfulMonad n] [Monad o] [LawfulMonad o] [AssertionLang l] [ExceptAssertionLang e] [WPMonad o l e]
+    [Monad n] [LawfulMonad n] [Monad o] [LawfulMonad o] [Assertion Pred] [Assertion EPred] [WP o Pred EPred]
     [MonadLiftT n o] [LawfulMonadLiftT n o] [Finite α Id]
     [IteratorLoop α Id o] [LawfulIteratorLoop α Id o]
     {it : Iter (α := α) β} {f : β → PostconditionT n (Option β₂)} {init : γ}
-    {g : β₂ → γ → o (ForInStep γ)} {P : l} {Q : γ → l} {eQ : e}
+    {g : β₂ → γ → o (ForInStep γ)} {P : Pred} {Q : γ → Pred} {eQ : EPred}
     (h : Triple P (forIn (m := o) it init (fun out acc => do
         match ← (f out).run with
         | some c => g c acc
@@ -1896,14 +1873,14 @@ theorem Spec.Iter.forIn_filterMapWithPostcondition {α β β₂ γ : Type w}
 @[lspec]
 theorem Spec.Iter.forIn_filterMapM {α β β₂ γ : Type w}
     {n : Type w → Type w'} {o : Type w → Type w''}
-    {l : Type w} {e : Type w}
+    {Pred : Type w} {EPred : Type w}
     [Iterator α Id β]
-    [Monad n] [LawfulMonad n] [Monad o] [LawfulMonad o] [AssertionLang l] [ExceptAssertionLang e] [WPMonad o l e]
+    [Monad n] [LawfulMonad n] [Monad o] [LawfulMonad o] [Assertion Pred] [Assertion EPred] [WP o Pred EPred]
     [MonadAttach n] [WeaklyLawfulMonadAttach n]
     [MonadLiftT n o] [LawfulMonadLiftT n o]
     [Finite α Id] [IteratorLoop α Id o] [LawfulIteratorLoop α Id o]
     {it : Iter (α := α) β} {f : β → n (Option β₂)} {init : γ} {g : β₂ → γ → o (ForInStep γ)}
-    {P : l} {Q : γ → l} {eQ : e}
+    {P : Pred} {Q : γ → Pred} {eQ : EPred}
     (h : Triple P (forIn (m := o) it init (fun out acc => do
         match ← f out with
         | some c => g c acc
@@ -1914,12 +1891,12 @@ theorem Spec.Iter.forIn_filterMapM {α β β₂ γ : Type w}
 @[lspec]
 theorem Spec.Iter.forIn_filterMap {α β β₂ γ : Type w}
     {n : Type w → Type w'}
-    {l : Type w} {e : Type w}
+    {Pred : Type w} {EPred : Type w}
     [Iterator α Id β]
-    [Monad n] [LawfulMonad n] [AssertionLang l] [ExceptAssertionLang e] [WPMonad n l e] [Finite α Id]
+    [Monad n] [LawfulMonad n] [Assertion Pred] [Assertion EPred] [WP n Pred EPred] [Finite α Id]
     [IteratorLoop α Id n] [LawfulIteratorLoop α Id n]
     {it : Iter (α := α) β} {f : β → Option β₂} {init : γ} {g : β₂ → γ → n (ForInStep γ)}
-    {P : l} {Q : γ → l} {eQ : e}
+    {P : Pred} {Q : γ → Pred} {eQ : EPred}
     (h : Triple P (forIn it init (fun out acc => do
         match f out with
         | some c => g c acc
@@ -1930,13 +1907,13 @@ theorem Spec.Iter.forIn_filterMap {α β β₂ γ : Type w}
 @[lspec]
 theorem Spec.Iter.forIn_mapWithPostcondition {α β β₂ γ : Type w}
     {n : Type w → Type w'} {o : Type w → Type w''}
-    {l : Type w} {e : Type w}
+    {Pred : Type w} {EPred : Type w}
     [Iterator α Id β]
-    [Monad n] [LawfulMonad n] [Monad o] [LawfulMonad o] [AssertionLang l] [ExceptAssertionLang e] [WPMonad o l e]
+    [Monad n] [LawfulMonad n] [Monad o] [LawfulMonad o] [Assertion Pred] [Assertion EPred] [WP o Pred EPred]
     [MonadLiftT n o] [LawfulMonadLiftT n o] [Finite α Id]
     [IteratorLoop α Id o] [LawfulIteratorLoop α Id o]
     {it : Iter (α := α) β} {f : β → PostconditionT n β₂} {init : γ}
-    {g : β₂ → γ → o (ForInStep γ)} {P : l} {Q : γ → l} {eQ : e}
+    {g : β₂ → γ → o (ForInStep γ)} {P : Pred} {Q : γ → Pred} {eQ : EPred}
     (h : Triple P (forIn (m := o) it init (fun out acc => do g (← (f out).run) acc)) Q eQ) :
     Triple P (forIn (it.mapWithPostcondition f) init g) Q eQ := by
   rwa [Std.Iter.forIn_mapWithPostcondition]
@@ -1944,15 +1921,15 @@ theorem Spec.Iter.forIn_mapWithPostcondition {α β β₂ γ : Type w}
 @[lspec]
 theorem Spec.Iter.forIn_mapM {α β β₂ γ : Type w}
     {n : Type w → Type w'} {o : Type w → Type w''}
-    {l : Type w} {e : Type w}
+    {Pred : Type w} {EPred : Type w}
     [Iterator α Id β]
-    [Monad n] [LawfulMonad n] [Monad o] [LawfulMonad o] [AssertionLang l] [ExceptAssertionLang e] [WPMonad o l e]
+    [Monad n] [LawfulMonad n] [Monad o] [LawfulMonad o] [Assertion Pred] [Assertion EPred] [WP o Pred EPred]
     [MonadAttach n] [WeaklyLawfulMonadAttach n]
     [MonadLiftT n o] [LawfulMonadLiftT n o]
     [Finite α Id]
     [IteratorLoop α Id o] [LawfulIteratorLoop α Id o]
     {it : Iter (α := α) β} {f : β → n β₂} {init : γ} {g : β₂ → γ → o (ForInStep γ)}
-    {P : l} {Q : γ → l} {eQ : e}
+    {P : Pred} {Q : γ → Pred} {eQ : EPred}
     (h : Triple P (forIn (m := o) it init (fun out acc => do g (← f out) acc)) Q eQ) :
     Triple P (forIn (it.mapM f) init g) Q eQ := by
   rwa [Std.Iter.forIn_mapM]
@@ -1960,12 +1937,12 @@ theorem Spec.Iter.forIn_mapM {α β β₂ γ : Type w}
 @[lspec]
 theorem Spec.Iter.forIn_map {α β β₂ γ : Type w}
     {n : Type w → Type w'}
-    {l : Type w} {e : Type w}
+    {Pred : Type w} {EPred : Type w}
     [Iterator α Id β]
-    [Monad n] [LawfulMonad n] [AssertionLang l] [ExceptAssertionLang e] [WPMonad n l e]
+    [Monad n] [LawfulMonad n] [Assertion Pred] [Assertion EPred] [WP n Pred EPred]
     [Finite α Id] [IteratorLoop α Id n] [LawfulIteratorLoop α Id n]
     {it : Iter (α := α) β} {f : β → β₂} {init : γ} {g : β₂ → γ → n (ForInStep γ)}
-    {P : l} {Q : γ → l} {eQ : e}
+    {P : Pred} {Q : γ → Pred} {eQ : EPred}
     (h : Triple P (forIn it init (fun out acc => do g (f out) acc)) Q eQ) :
     Triple P (forIn (it.map f) init g) Q eQ := by
   rwa [Std.Iter.forIn_map]
@@ -1973,13 +1950,13 @@ theorem Spec.Iter.forIn_map {α β β₂ γ : Type w}
 @[lspec]
 theorem Spec.Iter.forIn_filterWithPostcondition {α β γ : Type w}
     {n : Type w → Type w'} {o : Type w → Type w''}
-    {l : Type w} {e : Type w}
+    {Pred : Type w} {EPred : Type w}
     [Iterator α Id β]
-    [Monad n] [LawfulMonad n] [Monad o] [LawfulMonad o] [AssertionLang l] [ExceptAssertionLang e] [WPMonad o l e]
+    [Monad n] [LawfulMonad n] [Monad o] [LawfulMonad o] [Assertion Pred] [Assertion EPred] [WP o Pred EPred]
     [MonadLiftT n o] [LawfulMonadLiftT n o]
     [Finite α Id] [IteratorLoop α Id o] [LawfulIteratorLoop α Id o]
     {it : Iter (α := α) β} {f : β → PostconditionT n (ULift Bool)} {init : γ}
-    {g : β → γ → o (ForInStep γ)} {P : l} {Q : γ → l} {eQ : e}
+    {g : β → γ → o (ForInStep γ)} {P : Pred} {Q : γ → Pred} {eQ : EPred}
     (h : Triple P (forIn (m := o) it init (fun out acc => do if (← (f out).run).down then g out acc else return .yield acc)) Q eQ) :
     Triple P (forIn (it.filterWithPostcondition f) init g) Q eQ := by
   rwa [Std.Iter.forIn_filterWithPostcondition]
@@ -1987,14 +1964,14 @@ theorem Spec.Iter.forIn_filterWithPostcondition {α β γ : Type w}
 @[lspec]
 theorem Spec.Iter.forIn_filterM {α β γ : Type w}
     {n : Type w → Type w'} {o : Type w → Type w''}
-    {l : Type w} {e : Type w}
+    {Pred : Type w} {EPred : Type w}
     [Iterator α Id β]
-    [Monad n] [LawfulMonad n] [Monad o] [LawfulMonad o] [AssertionLang l] [ExceptAssertionLang e] [WPMonad o l e]
+    [Monad n] [LawfulMonad n] [Monad o] [LawfulMonad o] [Assertion Pred] [Assertion EPred] [WP o Pred EPred]
     [MonadAttach n] [WeaklyLawfulMonadAttach n]
     [MonadLiftT n o] [LawfulMonadLiftT n o] [Finite α Id]
     [IteratorLoop α Id o] [LawfulIteratorLoop α Id o]
     {it : Iter (α := α) β} {f : β → n (ULift Bool)} {init : γ} {g : β → γ → o (ForInStep γ)}
-    {P : l} {Q : γ → l} {eQ : e}
+    {P : Pred} {Q : γ → Pred} {eQ : EPred}
     (h : Triple P (forIn (m := o) it init (fun out acc => do if (← f out).down then g out acc else return .yield acc)) Q eQ) :
     Triple P (forIn (it.filterM f) init g) Q eQ := by
   rwa [Std.Iter.forIn_filterM]
@@ -2002,12 +1979,12 @@ theorem Spec.Iter.forIn_filterM {α β γ : Type w}
 @[lspec]
 theorem Spec.Iter.forIn_filter {α β γ : Type w}
     {n : Type w → Type w'}
-    {l : Type w} {e : Type w}
+    {Pred : Type w} {EPred : Type w}
     [Iterator α Id β]
-    [Monad n] [LawfulMonad n] [AssertionLang l] [ExceptAssertionLang e] [WPMonad n l e]
+    [Monad n] [LawfulMonad n] [Assertion Pred] [Assertion EPred] [WP n Pred EPred]
     [Finite α Id] [IteratorLoop α Id n] [LawfulIteratorLoop α Id n]
     {it : Iter (α := α) β} {f : β → Bool} {init : γ} {g : β → γ → n (ForInStep γ)}
-    {P : l} {Q : γ → l} {eQ : e}
+    {P : Pred} {Q : γ → Pred} {eQ : EPred}
     (h : Triple P (forIn it init (fun out acc => do if f out then g out acc else return .yield acc)) Q eQ) :
     Triple P (forIn (it.filter f) init g) Q eQ := by
   rwa [Std.Iter.forIn_filter]
@@ -2015,14 +1992,14 @@ theorem Spec.Iter.forIn_filter {α β γ : Type w}
 @[lspec]
 theorem Spec.Iter.foldM_filterMapWithPostcondition {α β γ δ : Type w}
     {n : Type w → Type w'} {o : Type w → Type w''}
-    {l : Type w} {e : Type w}
+    {Pred : Type w} {EPred : Type w}
     [Iterator α Id β] [Finite α Id]
-    [Monad n] [Monad o] [LawfulMonad n] [LawfulMonad o] [AssertionLang l] [ExceptAssertionLang e] [WPMonad o l e]
+    [Monad n] [Monad o] [LawfulMonad n] [LawfulMonad o] [Assertion Pred] [Assertion EPred] [WP o Pred EPred]
     [IteratorLoop α Id n] [IteratorLoop α Id o]
     [LawfulIteratorLoop α Id n] [LawfulIteratorLoop α Id o]
     [MonadLiftT n o] [LawfulMonadLiftT n o]
     {f : β → PostconditionT n (Option γ)} {g : δ → γ → o δ} {init : δ} {it : Iter (α := α) β}
-    {P : l} {Q : δ → l} {eQ : e}
+    {P : Pred} {Q : δ → Pred} {eQ : EPred}
     (h : Triple P (it.foldM (m := o) (init := init) (fun d b => do
           let some c ← (f b).run | Pure.pure d
           g d c)) Q eQ) :
@@ -2032,15 +2009,15 @@ theorem Spec.Iter.foldM_filterMapWithPostcondition {α β γ δ : Type w}
 @[lspec]
 theorem Spec.Iter.foldM_filterMapM {α β γ δ : Type w}
     {n : Type w → Type w'} {o : Type w → Type w''}
-    {l : Type w} {e : Type w}
+    {Pred : Type w} {EPred : Type w}
     [Iterator α Id β] [Finite α Id]
     [Monad n] [MonadAttach n] [LawfulMonad n] [WeaklyLawfulMonadAttach n]
-    [Monad o] [LawfulMonad o] [AssertionLang l] [ExceptAssertionLang e] [WPMonad o l e]
+    [Monad o] [LawfulMonad o] [Assertion Pred] [Assertion EPred] [WP o Pred EPred]
     [IteratorLoop α Id n] [IteratorLoop α Id o]
     [LawfulIteratorLoop α Id n] [LawfulIteratorLoop α Id o]
     [MonadLiftT n o] [LawfulMonadLiftT n o]
     {f : β → n (Option γ)} {g : δ → γ → o δ} {init : δ} {it : Iter (α := α) β}
-    {P : l} {Q : δ → l} {eQ : e}
+    {P : Pred} {Q : δ → Pred} {eQ : EPred}
     (h : Triple P (it.foldM (m := o) (init := init) (fun d b => do
           let some c ← f b | Pure.pure d
           g d c)) Q eQ) :
@@ -2050,14 +2027,14 @@ theorem Spec.Iter.foldM_filterMapM {α β γ δ : Type w}
 @[lspec]
 theorem Spec.Iter.foldM_mapWithPostcondition {α β γ δ : Type w}
     {m : Type w → Type w'''} {n : Type w → Type w'} {o : Type w → Type w''}
-    {l : Type w} {e : Type w}
+    {Pred : Type w} {EPred : Type w}
     [Iterator α Id β] [Finite α Id]
-    [Monad m] [Monad n] [Monad o] [LawfulMonad m] [LawfulMonad n] [LawfulMonad o] [AssertionLang l] [ExceptAssertionLang e] [WPMonad o l e]
+    [Monad m] [Monad n] [Monad o] [LawfulMonad m] [LawfulMonad n] [LawfulMonad o] [Assertion Pred] [Assertion EPred] [WP o Pred EPred]
     [IteratorLoop α Id n] [IteratorLoop α Id o]
     [LawfulIteratorLoop α Id n] [LawfulIteratorLoop α Id o]
     [MonadLiftT n o] [LawfulMonadLiftT n o]
     {f : β → PostconditionT n γ} {g : δ → γ → o δ} {init : δ} {it : Iter (α := α) β}
-    {P : l} {Q : δ → l} {eQ : e}
+    {P : Pred} {Q : δ → Pred} {eQ : EPred}
     (h : Triple P (it.foldM (m := o) (init := init) (fun d b => do let c ← (f b).run; g d c)) Q eQ) :
     Triple P ((it.mapWithPostcondition f).foldM (init := init) g) Q eQ := by
   rwa [Std.Iter.foldM_mapWithPostcondition (m := m)]
@@ -2065,15 +2042,15 @@ theorem Spec.Iter.foldM_mapWithPostcondition {α β γ δ : Type w}
 @[lspec]
 theorem Spec.Iter.foldM_mapM {α β γ δ : Type w}
     {n : Type w → Type w'} {o : Type w → Type w''}
-    {l : Type w} {e : Type w}
+    {Pred : Type w} {EPred : Type w}
     [Iterator α Id β] [Finite α Id]
     [Monad n] [MonadAttach n] [LawfulMonad n] [WeaklyLawfulMonadAttach n]
-    [Monad o] [LawfulMonad o] [AssertionLang l] [ExceptAssertionLang e] [WPMonad o l e]
+    [Monad o] [LawfulMonad o] [Assertion Pred] [Assertion EPred] [WP o Pred EPred]
     [IteratorLoop α Id n] [IteratorLoop α Id o]
     [LawfulIteratorLoop α Id n] [LawfulIteratorLoop α Id o]
     [MonadLiftT n o] [LawfulMonadLiftT n o]
     {f : β → n γ} {g : δ → γ → o δ} {init : δ} {it : Iter (α := α) β}
-    {P : l} {Q : δ → l} {eQ : e}
+    {P : Pred} {Q : δ → Pred} {eQ : EPred}
     (h : Triple P (it.foldM (m := o) (init := init) (fun d b => do let c ← f b; g d c)) Q eQ) :
     Triple P ((it.mapM f).foldM (init := init) g) Q eQ := by
   rwa [Std.Iter.foldM_mapM]
@@ -2081,14 +2058,14 @@ theorem Spec.Iter.foldM_mapM {α β γ δ : Type w}
 @[lspec]
 theorem Spec.Iter.foldM_filterWithPostcondition {α β δ : Type w}
     {n : Type w → Type w'} {o : Type w → Type w''}
-    {l : Type w} {e : Type w}
+    {Pred : Type w} {EPred : Type w}
     [Iterator α Id β] [Finite α Id]
-    [Monad n] [Monad o] [LawfulMonad n] [LawfulMonad o] [AssertionLang l] [ExceptAssertionLang e] [WPMonad o l e]
+    [Monad n] [Monad o] [LawfulMonad n] [LawfulMonad o] [Assertion Pred] [Assertion EPred] [WP o Pred EPred]
     [IteratorLoop α Id n] [IteratorLoop α Id o]
     [LawfulIteratorLoop α Id n] [LawfulIteratorLoop α Id o]
     [MonadLiftT n o] [LawfulMonadLiftT n o]
     {f : β → PostconditionT n (ULift Bool)} {g : δ → β → o δ} {init : δ} {it : Iter (α := α) β}
-    {P : l} {Q : δ → l} {eQ : e}
+    {P : Pred} {Q : δ → Pred} {eQ : EPred}
     (h : Triple P (it.foldM (m := o) (init := init) (fun d b => do if (← (f b).run).down then g d b else Pure.pure d)) Q eQ) :
     Triple P ((it.filterWithPostcondition f).foldM (init := init) g) Q eQ := by
   rwa [Std.Iter.foldM_filterWithPostcondition]
@@ -2096,15 +2073,15 @@ theorem Spec.Iter.foldM_filterWithPostcondition {α β δ : Type w}
 @[lspec]
 theorem Spec.Iter.foldM_filterM {α β δ : Type w}
     {n : Type w → Type w'} {o : Type w → Type w''}
-    {l : Type w} {e : Type w}
+    {Pred : Type w} {EPred : Type w}
     [Iterator α Id β] [Finite α Id]
     [Monad n] [MonadAttach n] [LawfulMonad n] [WeaklyLawfulMonadAttach n]
-    [Monad o] [LawfulMonad o] [AssertionLang l] [ExceptAssertionLang e] [WPMonad o l e]
+    [Monad o] [LawfulMonad o] [Assertion Pred] [Assertion EPred] [WP o Pred EPred]
     [IteratorLoop α Id n] [IteratorLoop α Id o]
     [LawfulIteratorLoop α Id n] [LawfulIteratorLoop α Id o]
     [MonadLiftT n o] [LawfulMonadLiftT n o]
     {f : β → n (ULift Bool)} {g : δ → β → o δ} {init : δ} {it : Iter (α := α) β}
-    {P : l} {Q : δ → l} {eQ : e}
+    {P : Pred} {Q : δ → Pred} {eQ : EPred}
     (h : Triple P (it.foldM (m := o) (init := init) (fun d b => do if (← f b).down then g d b else Pure.pure d)) Q eQ) :
     Triple P ((it.filterM f).foldM (init := init) g) Q eQ := by
   rwa [Std.Iter.foldM_filterM]
@@ -2112,12 +2089,12 @@ theorem Spec.Iter.foldM_filterM {α β δ : Type w}
 @[lspec]
 theorem Spec.Iter.foldM_filterMap {α β γ δ : Type w}
     {n : Type w → Type w'}
-    {l : Type w} {e : Type w}
-    [Iterator α Id β] [Finite α Id] [Monad n] [LawfulMonad n] [AssertionLang l] [ExceptAssertionLang e] [WPMonad n l e]
+    {Pred : Type w} {EPred : Type w}
+    [Iterator α Id β] [Finite α Id] [Monad n] [LawfulMonad n] [Assertion Pred] [Assertion EPred] [WP n Pred EPred]
     [IteratorLoop α Id n]
     [LawfulIteratorLoop α Id n]
     {f : β → Option γ} {g : δ → γ → n δ} {init : δ} {it : Iter (α := α) β}
-    {P : l} {Q : δ → l} {eQ : e}
+    {P : Pred} {Q : δ → Pred} {eQ : EPred}
     (h : Triple P (it.foldM (init := init) (fun d b => do
           let some c := f b | Pure.pure d
           g d c)) Q eQ) :
@@ -2127,11 +2104,11 @@ theorem Spec.Iter.foldM_filterMap {α β γ δ : Type w}
 @[lspec]
 theorem Spec.Iter.foldM_map {α β γ δ : Type w}
     {n : Type w → Type w'}
-    {l : Type w} {e : Type w}
-    [Iterator α Id β] [Finite α Id] [Monad n] [LawfulMonad n] [AssertionLang l] [ExceptAssertionLang e] [WPMonad n l e]
+    {Pred : Type w} {EPred : Type w}
+    [Iterator α Id β] [Finite α Id] [Monad n] [LawfulMonad n] [Assertion Pred] [Assertion EPred] [WP n Pred EPred]
     [IteratorLoop α Id n] [LawfulIteratorLoop α Id n]
     {f : β → γ} {g : δ → γ → n δ} {init : δ} {it : Iter (α := α) β}
-    {P : l} {Q : δ → l} {eQ : e}
+    {P : Pred} {Q : δ → Pred} {eQ : EPred}
     (h : Triple P (it.foldM (init := init) (fun d b => do g d (f b))) Q eQ) :
     Triple P ((it.map f).foldM (init := init) g) Q eQ := by
   rwa [Std.Iter.foldM_map]
@@ -2139,11 +2116,11 @@ theorem Spec.Iter.foldM_map {α β γ δ : Type w}
 @[lspec]
 theorem Spec.Iter.foldM_filter {α β δ : Type w}
     {n : Type w → Type w'}
-    {l : Type w} {e : Type w}
-    [Iterator α Id β] [Finite α Id] [Monad n] [LawfulMonad n] [AssertionLang l] [ExceptAssertionLang e] [WPMonad n l e]
+    {Pred : Type w} {EPred : Type w}
+    [Iterator α Id β] [Finite α Id] [Monad n] [LawfulMonad n] [Assertion Pred] [Assertion EPred] [WP n Pred EPred]
     [IteratorLoop α Id n] [LawfulIteratorLoop α Id n]
     {f : β → Bool} {g : δ → β → n δ} {init : δ} {it : Iter (α := α) β}
-    {P : l} {Q : δ → l} {eQ : e}
+    {P : Pred} {Q : δ → Pred} {eQ : EPred}
     (h : Triple P (it.foldM (init := init) (fun d b => if f b then g d b else Pure.pure d)) Q eQ) :
     Triple P ((it.filter f).foldM (init := init) g) Q eQ := by
   rwa [Std.Iter.foldM_filter]
@@ -2151,12 +2128,12 @@ theorem Spec.Iter.foldM_filter {α β δ : Type w}
 @[lspec]
 theorem Spec.Iter.fold_filterMapWithPostcondition {α β γ δ : Type w}
     {n : Type w → Type w'}
-    {l : Type w} {e : Type w}
+    {Pred : Type w} {EPred : Type w}
     [Iterator α Id β] [Finite α Id]
-    [Monad n] [LawfulMonad n] [AssertionLang l] [ExceptAssertionLang e] [WPMonad n l e]
+    [Monad n] [LawfulMonad n] [Assertion Pred] [Assertion EPred] [WP n Pred EPred]
     [IteratorLoop α Id n] [LawfulIteratorLoop α Id n]
     {f : β → PostconditionT n (Option γ)} {g : δ → γ → δ} {init : δ} {it : Iter (α := α) β}
-    {P : l} {Q : δ → l} {eQ : e}
+    {P : Pred} {Q : δ → Pred} {eQ : EPred}
     (h : Triple P (it.foldM (init := init) (fun d b => do
           let some c ← (f b).run | Pure.pure d
           return g d c)) Q eQ) :
@@ -2166,12 +2143,12 @@ theorem Spec.Iter.fold_filterMapWithPostcondition {α β γ δ : Type w}
 @[lspec]
 theorem Spec.Iter.fold_filterMapM {α β γ δ : Type w}
     {n : Type w → Type w'}
-    {l : Type w} {e : Type w}
+    {Pred : Type w} {EPred : Type w}
     [Iterator α Id β] [Finite α Id]
-    [Monad n] [MonadAttach n] [LawfulMonad n] [WeaklyLawfulMonadAttach n] [AssertionLang l] [ExceptAssertionLang e] [WPMonad n l e]
+    [Monad n] [MonadAttach n] [LawfulMonad n] [WeaklyLawfulMonadAttach n] [Assertion Pred] [Assertion EPred] [WP n Pred EPred]
     [IteratorLoop α Id n] [LawfulIteratorLoop α Id n]
     {f : β → n (Option γ)} {g : δ → γ → δ} {init : δ} {it : Iter (α := α) β}
-    {P : l} {Q : δ → l} {eQ : e}
+    {P : Pred} {Q : δ → Pred} {eQ : EPred}
     (h : Triple P (it.foldM (init := init) (fun d b => do
           let some c ← f b | Pure.pure d
           return g d c)) Q eQ) :
@@ -2181,12 +2158,12 @@ theorem Spec.Iter.fold_filterMapM {α β γ δ : Type w}
 @[lspec]
 theorem Spec.Iter.fold_mapWithPostcondition {α β γ δ : Type w}
     {n : Type w → Type w'}
-    {l : Type w} {e : Type w}
+    {Pred : Type w} {EPred : Type w}
     [Iterator α Id β] [Finite α Id]
-    [Monad n] [LawfulMonad n] [AssertionLang l] [ExceptAssertionLang e] [WPMonad n l e]
+    [Monad n] [LawfulMonad n] [Assertion Pred] [Assertion EPred] [WP n Pred EPred]
     [IteratorLoop α Id n] [LawfulIteratorLoop α Id n]
     {f : β → PostconditionT n γ} {g : δ → γ → δ} {init : δ} {it : Iter (α := α) β}
-    {P : l} {Q : δ → l} {eQ : e}
+    {P : Pred} {Q : δ → Pred} {eQ : EPred}
     (h : Triple P (it.foldM (init := init) (fun d b => do let c ← (f b).run; return g d c)) Q eQ) :
     Triple P ((it.mapWithPostcondition f).fold (init := init) g) Q eQ := by
   rwa [Std.Iter.fold_mapWithPostcondition]
@@ -2194,12 +2171,12 @@ theorem Spec.Iter.fold_mapWithPostcondition {α β γ δ : Type w}
 @[lspec]
 theorem Spec.Iter.fold_mapM {α β γ δ : Type w}
     {n : Type w → Type w'}
-    {l : Type w} {e : Type w}
+    {Pred : Type w} {EPred : Type w}
     [Iterator α Id β] [Finite α Id]
-    [Monad n] [MonadAttach n] [LawfulMonad n] [WeaklyLawfulMonadAttach n] [AssertionLang l] [ExceptAssertionLang e] [WPMonad n l e]
+    [Monad n] [MonadAttach n] [LawfulMonad n] [WeaklyLawfulMonadAttach n] [Assertion Pred] [Assertion EPred] [WP n Pred EPred]
     [IteratorLoop α Id n] [LawfulIteratorLoop α Id n]
     {f : β → n γ} {g : δ → γ → δ} {init : δ} {it : Iter (α := α) β}
-    {P : l} {Q : δ → l} {eQ : e}
+    {P : Pred} {Q : δ → Pred} {eQ : EPred}
     (h : Triple P (it.foldM (init := init) (fun d b => do let c ← f b; return g d c)) Q eQ) :
     Triple P ((it.mapM f).fold (init := init) g) Q eQ := by
   rwa [Std.Iter.fold_mapM]
@@ -2207,12 +2184,12 @@ theorem Spec.Iter.fold_mapM {α β γ δ : Type w}
 @[lspec]
 theorem Spec.Iter.fold_filterWithPostcondition {α β δ : Type w}
     {n : Type w → Type w'}
-    {l : Type w} {e : Type w}
+    {Pred : Type w} {EPred : Type w}
     [Iterator α Id β] [Finite α Id]
-    [Monad n] [LawfulMonad n] [AssertionLang l] [ExceptAssertionLang e] [WPMonad n l e]
+    [Monad n] [LawfulMonad n] [Assertion Pred] [Assertion EPred] [WP n Pred EPred]
     [IteratorLoop α Id n] [LawfulIteratorLoop α Id n]
     {f : β → PostconditionT n (ULift Bool)} {g : δ → β → δ} {init : δ} {it : Iter (α := α) β}
-    {P : l} {Q : δ → l} {eQ : e}
+    {P : Pred} {Q : δ → Pred} {eQ : EPred}
     (h : Triple P (it.foldM (init := init) (fun d b => return if (← (f b).run).down then g d b else d)) Q eQ) :
     Triple P ((it.filterWithPostcondition f).fold (init := init) g) Q eQ := by
   rwa [Std.Iter.fold_filterWithPostcondition]
@@ -2220,12 +2197,12 @@ theorem Spec.Iter.fold_filterWithPostcondition {α β δ : Type w}
 @[lspec]
 theorem Spec.Iter.fold_filterM {α β δ : Type w}
     {n : Type w → Type w'}
-    {l : Type w} {e : Type w}
+    {Pred : Type w} {EPred : Type w}
     [Iterator α Id β] [Finite α Id]
-    [Monad n] [MonadAttach n] [LawfulMonad n] [WeaklyLawfulMonadAttach n] [AssertionLang l] [ExceptAssertionLang e] [WPMonad n l e]
+    [Monad n] [MonadAttach n] [LawfulMonad n] [WeaklyLawfulMonadAttach n] [Assertion Pred] [Assertion EPred] [WP n Pred EPred]
     [IteratorLoop α Id n] [LawfulIteratorLoop α Id n]
     {f : β → n (ULift Bool)} {g : δ → β → δ} {init : δ} {it : Iter (α := α) β}
-    {P : l} {Q : δ → l} {eQ : e}
+    {P : Pred} {Q : δ → Pred} {eQ : EPred}
     (h : Triple P (it.foldM (init := init) (fun d b => return if (← f b).down then g d b else d)) Q eQ) :
     Triple P ((it.filterM f).fold (init := init) g) Q eQ := by
   rwa [Std.Iter.fold_filterM]
@@ -2235,8 +2212,8 @@ end Iterators
 
 @[lspec]
 theorem Spec.forIn'_array {xs : Array α} {init : β} {f : (a : α) → a ∈ xs → β → m (ForInStep β)}
-    (inv : Invariant xs.toList β l)
-    (eInv : e)
+    (inv : Invariant xs.toList β Pred)
+    (eInv : EPred)
     (step : ∀ pref cur suff (h : xs.toList = pref ++ cur :: suff) b,
       Triple
         (inv (⟨pref, cur::suff, h.symm⟩, b))
@@ -2254,8 +2231,8 @@ theorem Spec.forIn'_array {xs : Array α} {init : β} {f : (a : α) → a ∈ xs
 
 @[lspec]
 theorem Spec.forIn_array {xs : Array α} {init : β} {f : α → β → m (ForInStep β)}
-    (inv : Invariant xs.toList β l)
-    (eInv : e)
+    (inv : Invariant xs.toList β Pred)
+    (eInv : EPred)
     (step : ∀ pref cur suff (h : xs.toList = pref ++ cur :: suff) b,
       Triple
         (inv (⟨pref, cur::suff, h.symm⟩, b))
@@ -2274,8 +2251,8 @@ theorem Spec.forIn_array {xs : Array α} {init : β} {f : α → β → m (ForIn
 @[lspec]
 theorem Spec.foldlM_array [LawfulMonad m]
     {xs : Array α} {init : β} {f : β → α → m β}
-    (inv : Invariant xs.toList β l)
-    (eInv : e)
+    (inv : Invariant xs.toList β Pred)
+    (eInv : EPred)
     (step : ∀ pref cur suff (h : xs.toList = pref ++ cur :: suff) b,
       Triple
         (inv (⟨pref, cur::suff, h.symm⟩, b))
