Loom/Instances/Rand.lean
@@ -6,41 +6,41 @@ import Plausible.Testable
 
 open Lean.Order Loom
 
-instance (priority := high) {σ : Type} {m : Type → Type v} [Monad m] [LawfulMonad m] [WPMonad m Prop e] [Inhabited σ] :
-  WPMonad (StateT σ m) Prop e where
+instance (priority := high) {σ : Type} {m : Type → Type v} [Monad m] [LawfulMonad m] [WP m Prop EPred] [Inhabited σ] :
+  WP (StateT σ m) Prop EPred where
   wpImpl x post epost := ∀ s, wp (m := m) (x s) (fun p => post p.1) epost
   wp_pure_impl x post epost := by
     intro hx s
-    exact (WPMonad.wp_pure (m := m) (x := (x, s)) (post := fun p => post p.1) (epost := epost)) hx
+    exact (WP.wp_pure (m := m) (x := (x, s)) (post := fun p => post p.1) (epost := epost)) hx
   wp_bind_impl x f post epost := by
-    intro wph s; apply WPMonad.wp_bind (m := m)
-    apply WPMonad.wp_cons (m := m); rotate_left; apply wph
+    intro wph s; apply WP.wp_bind (m := m)
+    apply WP.wp_consequence (m := m); rotate_left; apply wph
     intro x h; simp_all
-  wp_cons_impl x post post' epost h := by
-    intro s s'; apply WPMonad.wp_cons (m := m);
+  wp_consequence_impl x post post' epost h := by
+    intro s s'; apply WP.wp_consequence (m := m);
     intro x; apply h; solve_by_elim
 
-instance (priority := high) [Monad m] [LawfulMonad m] [WPMonad m Prop e] [Inhabited ρ] :
-  WPMonad (ReaderT ρ m) Prop e where
+instance (priority := high) [Monad m] [LawfulMonad m] [WP m Prop EPred] [Inhabited ρ] :
+  WP (ReaderT ρ m) Prop EPred where
   wpImpl x post epost := ∀ r, wp (m := m) (x r) post epost
   wp_pure_impl x post epost := by
     intro hx r
-    exact (WPMonad.wp_pure (m := m) (x := x) (post := post) (epost := epost)) hx
+    exact (WP.wp_pure (m := m) (x := x) (post := post) (epost := epost)) hx
   wp_bind_impl x f post epost := by
-    intro wph r; apply WPMonad.wp_bind (m := m)
-    apply WPMonad.wp_cons (m := m); rotate_left; apply wph
+    intro wph r; apply WP.wp_bind (m := m)
+    apply WP.wp_consequence (m := m); rotate_left; apply wph
     intro x h; simp_all
-  wp_cons_impl x post post' epost h := by
-    intro r r'; apply WPMonad.wp_cons (m := m);
+  wp_consequence_impl x post post' epost h := by
+    intro r r'; apply WP.wp_consequence (m := m);
     intro x; apply h; solve_by_elim
 
-instance (priority := high) : WPMonad (Except ε) Prop PUnit where
+instance (priority := high) : WP (Except ε) Prop PUnit where
   wpImpl x post epost := match x with
     | .ok x => post x
     | .error e => False
   wp_pure_impl x post epost := PartialOrder.rel_refl
   wp_bind_impl x f post epost := by cases x <;> exact id
-  wp_cons_impl x post post' epost h := by cases x with
+  wp_consequence_impl x post post' epost h := by cases x with
     | ok a => exact h a
     | error e => exact id
 
@@ -56,15 +56,15 @@ theorem chooseAny_wp (post : α → Prop) [Random Id α] :
 theorem Testable.run_wp [Testable p] c m :
   Triple (p ∧ post) (Testable.runPropE p c m) (fun _ => post) ⟨⟩ := by
   rw [Triple.iff]; intro ⟨ph, posth⟩
-  simp [Testable.runPropE]; apply WPMonad.wp_bind (m := Gen)
+  simp [Testable.runPropE]; apply WP.wp_bind (m := Gen)
   simp [tryCatch, MonadExceptOf.tryCatch, tryCatchThe, Except.tryCatch]
   intro s r; simp
   split
-  { simp only [wp, WPMonad.wpImpl]
+  { simp only [wp, WP.wpImpl]
     intro s r; split; solve_by_elim
     rename_i a _ _ _ _
     rcases a with ⟨⟨⟩, _⟩ <;> try simp_all [Functor.map, StateT.map, pure, StateT.pure, Except.pure, ReaderT.pure] }
   have hgave : wp (pure (TestResult.gaveUp 1) : Gen (TestResult p)) (fun _ => post) PUnit.unit :=
-    (WPMonad.wp_pure (m := Gen) (x := TestResult.gaveUp 1)
+    (WP.wp_pure (m := Gen) (x := TestResult.gaveUp 1)
       (post := fun _ => post) (epost := PUnit.unit)) posth
   simpa [pure, StateT.pure, ReaderT.pure] using hgave
